Completeness in detail Reorganized theory structure

Hygge_Theory.thy
@@ -1,178 +1,131 @@
 theory Hygge_Theory
 imports
-  "Operational"
-  "Denotational"
+  "Coinductive_Prop"
 
 begin
 
-(* To start solving specification [\<Psi>], we start at configuration [], 0 \<turnstile> \<Psi> \<triangleright> [] *)
+section \<open>Initial configuration\<close>
+
 lemma solve_start:
-  shows "\<lbrakk>\<lbrakk> \<Psi> \<rbrakk>\<rbrakk>\<^sub>T\<^sub>E\<^sub>S\<^sub>L = \<lbrakk> [], 0 \<turnstile> \<Psi> \<triangleright> [] \<rbrakk>\<^sub>c\<^sub>o\<^sub>n\<^sub>f"
+  shows "\<lbrakk>\<lbrakk> \<Psi> \<rbrakk>\<rbrakk>\<^sub>T\<^sub>E\<^sub>S\<^sub>L = \<lbrakk> [], 0 \<turnstile> \<Psi> \<triangleright> [] \<rbrakk>\<^sub>c\<^sub>o\<^sub>n\<^sub>f\<^sub>i\<^sub>g"
   proof -
-    have "\<lbrakk>\<lbrakk> \<Psi> \<rbrakk>\<rbrakk>\<^sub>T\<^sub>E\<^sub>S\<^sub>L = \<lbrakk>\<lbrakk> \<Psi> \<nabla> 0 \<rbrakk>\<rbrakk>\<^sub>T\<^sub>E\<^sub>S\<^sub>L"
+    have "\<lbrakk>\<lbrakk> \<Psi> \<rbrakk>\<rbrakk>\<^sub>T\<^sub>E\<^sub>S\<^sub>L = \<lbrakk>\<lbrakk> \<Psi> \<rbrakk>\<rbrakk>\<^sub>T\<^sub>E\<^sub>S\<^sub>L\<^bsup>\<ge> 0\<^esup>"
     by (simp add: TESL_interpretation_at_index_zero')
-    moreover have "\<lbrakk> [], 0 \<turnstile> \<Psi> \<triangleright> [] \<rbrakk>\<^sub>c\<^sub>o\<^sub>n\<^sub>f = \<lbrakk>\<lbrakk> [] \<rbrakk>\<rbrakk>\<^sub>s\<^sub>y\<^sub>m\<^sub>r\<^sub>u\<^sub>n \<inter> \<lbrakk>\<lbrakk> \<Psi> \<nabla> 0 \<rbrakk>\<rbrakk>\<^sub>T\<^sub>E\<^sub>S\<^sub>L \<inter> \<lbrakk>\<lbrakk> [] \<nabla> Suc 0 \<rbrakk>\<rbrakk>\<^sub>T\<^sub>E\<^sub>S\<^sub>L"
+    moreover have "\<lbrakk> [], 0 \<turnstile> \<Psi> \<triangleright> [] \<rbrakk>\<^sub>c\<^sub>o\<^sub>n\<^sub>f\<^sub>i\<^sub>g = \<lbrakk>\<lbrakk> [] \<rbrakk>\<rbrakk>\<^sub>s\<^sub>y\<^sub>m\<^sub>r\<^sub>u\<^sub>n \<inter> \<lbrakk>\<lbrakk> \<Psi> \<rbrakk>\<rbrakk>\<^sub>T\<^sub>E\<^sub>S\<^sub>L\<^bsup>\<ge> 0\<^esup> \<inter> \<lbrakk>\<lbrakk> [] \<rbrakk>\<rbrakk>\<^sub>T\<^sub>E\<^sub>S\<^sub>L\<^bsup>\<ge> Suc 0\<^esup>"
     by simp
     ultimately show ?thesis by auto
   qed
 
-(**) section \<open>Soundness\<close> (**)
+section \<open>Soundness\<close>
 
 theorem soundness:
   assumes "\<Gamma>\<^sub>1, n\<^sub>1 \<turnstile> \<Psi>\<^sub>1 \<triangleright> \<Phi>\<^sub>1  \<hookrightarrow>  \<Gamma>\<^sub>2, n\<^sub>2 \<turnstile> \<Psi>\<^sub>2 \<triangleright> \<Phi>\<^sub>2"
-  shows "\<lbrakk>\<lbrakk> \<Gamma>\<^sub>1 \<rbrakk>\<rbrakk>\<^sub>s\<^sub>y\<^sub>m\<^sub>r\<^sub>u\<^sub>n \<inter> \<lbrakk>\<lbrakk> \<Psi>\<^sub>1 \<nabla> n\<^sub>1 \<rbrakk>\<rbrakk>\<^sub>T\<^sub>E\<^sub>S\<^sub>L \<inter> \<lbrakk>\<lbrakk> \<Phi>\<^sub>1 \<nabla> Suc n\<^sub>1 \<rbrakk>\<rbrakk>\<^sub>T\<^sub>E\<^sub>S\<^sub>L
-          \<supseteq>  \<lbrakk>\<lbrakk> \<Gamma>\<^sub>2 \<rbrakk>\<rbrakk>\<^sub>s\<^sub>y\<^sub>m\<^sub>r\<^sub>u\<^sub>n \<inter> \<lbrakk>\<lbrakk> \<Psi>\<^sub>2 \<nabla> n\<^sub>2 \<rbrakk>\<rbrakk>\<^sub>T\<^sub>E\<^sub>S\<^sub>L \<inter> \<lbrakk>\<lbrakk> \<Phi>\<^sub>2 \<nabla> Suc n\<^sub>2 \<rbrakk>\<rbrakk>\<^sub>T\<^sub>E\<^sub>S\<^sub>L"
+  shows "\<lbrakk>\<lbrakk> \<Gamma>\<^sub>1 \<rbrakk>\<rbrakk>\<^sub>s\<^sub>y\<^sub>m\<^sub>r\<^sub>u\<^sub>n \<inter> \<lbrakk>\<lbrakk> \<Psi>\<^sub>1 \<rbrakk>\<rbrakk>\<^sub>T\<^sub>E\<^sub>S\<^sub>L\<^bsup>\<ge> n\<^sub>1\<^esup> \<inter> \<lbrakk>\<lbrakk> \<Phi>\<^sub>1 \<rbrakk>\<rbrakk>\<^sub>T\<^sub>E\<^sub>S\<^sub>L\<^bsup>\<ge> Suc n\<^sub>1\<^esup>
+          \<supseteq>  \<lbrakk>\<lbrakk> \<Gamma>\<^sub>2 \<rbrakk>\<rbrakk>\<^sub>s\<^sub>y\<^sub>m\<^sub>r\<^sub>u\<^sub>n \<inter> \<lbrakk>\<lbrakk> \<Psi>\<^sub>2 \<rbrakk>\<rbrakk>\<^sub>T\<^sub>E\<^sub>S\<^sub>L\<^bsup>\<ge> n\<^sub>2\<^esup> \<inter> \<lbrakk>\<lbrakk> \<Phi>\<^sub>2 \<rbrakk>\<rbrakk>\<^sub>T\<^sub>E\<^sub>S\<^sub>L\<^bsup>\<ge> Suc n\<^sub>2\<^esup>"
   proof (insert assms, erule operational_semantics_step.cases)
-  show "\<And>\<Gamma> n \<Phi>.
-       (\<Gamma>\<^sub>1, n\<^sub>1 \<turnstile> \<Psi>\<^sub>1 \<triangleright> \<Phi>\<^sub>1) = (\<Gamma>, n \<turnstile> [] \<triangleright> \<Phi>) \<Longrightarrow>
-       (\<Gamma>\<^sub>2, n\<^sub>2 \<turnstile> \<Psi>\<^sub>2 \<triangleright> \<Phi>\<^sub>2) = (\<Gamma>, Suc n \<turnstile> \<Phi> \<triangleright> []) \<Longrightarrow>
-       (* consistent_run \<Gamma> \<Longrightarrow> *)
-       \<lbrakk>\<lbrakk> \<Gamma>\<^sub>2 \<rbrakk>\<rbrakk>\<^sub>s\<^sub>y\<^sub>m\<^sub>r\<^sub>u\<^sub>n \<inter> \<lbrakk>\<lbrakk> \<Psi>\<^sub>2 \<nabla> n\<^sub>2 \<rbrakk>\<rbrakk>\<^sub>T\<^sub>E\<^sub>S\<^sub>L \<inter> \<lbrakk>\<lbrakk> \<Phi>\<^sub>2 \<nabla> Suc n\<^sub>2 \<rbrakk>\<rbrakk>\<^sub>T\<^sub>E\<^sub>S\<^sub>L \<subseteq> \<lbrakk>\<lbrakk> \<Gamma>\<^sub>1 \<rbrakk>\<rbrakk>\<^sub>s\<^sub>y\<^sub>m\<^sub>r\<^sub>u\<^sub>n \<inter> \<lbrakk>\<lbrakk> \<Psi>\<^sub>1 \<nabla> n\<^sub>1 \<rbrakk>\<rbrakk>\<^sub>T\<^sub>E\<^sub>S\<^sub>L \<inter> \<lbrakk>\<lbrakk> \<Phi>\<^sub>1 \<nabla> Suc n\<^sub>1 \<rbrakk>\<rbrakk>\<^sub>T\<^sub>E\<^sub>S\<^sub>L"
-    by auto
-  show "\<And>\<Gamma> n K \<tau> \<Psi> \<Phi>.
-       (\<Gamma>\<^sub>1, n\<^sub>1 \<turnstile> \<Psi>\<^sub>1 \<triangleright> \<Phi>\<^sub>1) = (\<Gamma>, n \<turnstile> (K sporadic \<tau>) # \<Psi> \<triangleright> \<Phi>) \<Longrightarrow>
-       (\<Gamma>\<^sub>2, n\<^sub>2 \<turnstile> \<Psi>\<^sub>2 \<triangleright> \<Phi>\<^sub>2) = (\<Gamma>, n \<turnstile> \<Psi> \<triangleright> (K sporadic \<tau>) # \<Phi>) \<Longrightarrow>
-       (* consistent_run \<Gamma> \<Longrightarrow> *)
-       \<lbrakk>\<lbrakk> \<Gamma>\<^sub>2 \<rbrakk>\<rbrakk>\<^sub>s\<^sub>y\<^sub>m\<^sub>r\<^sub>u\<^sub>n \<inter> \<lbrakk>\<lbrakk> \<Psi>\<^sub>2 \<nabla> n\<^sub>2 \<rbrakk>\<rbrakk>\<^sub>T\<^sub>E\<^sub>S\<^sub>L \<inter> \<lbrakk>\<lbrakk> \<Phi>\<^sub>2 \<nabla> Suc n\<^sub>2 \<rbrakk>\<rbrakk>\<^sub>T\<^sub>E\<^sub>S\<^sub>L \<subseteq> \<lbrakk>\<lbrakk> \<Gamma>\<^sub>1 \<rbrakk>\<rbrakk>\<^sub>s\<^sub>y\<^sub>m\<^sub>r\<^sub>u\<^sub>n \<inter> \<lbrakk>\<lbrakk> \<Psi>\<^sub>1 \<nabla> n\<^sub>1 \<rbrakk>\<rbrakk>\<^sub>T\<^sub>E\<^sub>S\<^sub>L \<inter> \<lbrakk>\<lbrakk> \<Phi>\<^sub>1 \<nabla> Suc n\<^sub>1 \<rbrakk>\<rbrakk>\<^sub>T\<^sub>E\<^sub>S\<^sub>L"
-    using TESL_interp_at_index_sporadic_cases
-    by (smt Int_subset_iff Pair_inject TESL_interpretation_at_index_cons_morph inf.cobounded1 inf.cobounded2 subset_trans sup.cobounded2)
-  show "\<And>K n \<tau> \<Gamma> \<Psi> \<Phi>.
-       (\<Gamma>\<^sub>1, n\<^sub>1 \<turnstile> \<Psi>\<^sub>1 \<triangleright> \<Phi>\<^sub>1) = (\<Gamma>, n \<turnstile> (K sporadic \<tau>) # \<Psi> \<triangleright> \<Phi>) \<Longrightarrow>
-       (\<Gamma>\<^sub>2, n\<^sub>2 \<turnstile> \<Psi>\<^sub>2 \<triangleright> \<Phi>\<^sub>2) = (K \<Up> n # K \<Down> n @ \<lfloor> \<tau> \<rfloor> # \<Gamma>, n \<turnstile> \<Psi> \<triangleright> \<Phi>) \<Longrightarrow>
-       (* consistent_run (K \<Up> n # K \<Down> n @ \<lfloor> \<tau> \<rfloor> # \<Gamma>) \<Longrightarrow> *)
-       \<lbrakk>\<lbrakk> \<Gamma>\<^sub>2 \<rbrakk>\<rbrakk>\<^sub>s\<^sub>y\<^sub>m\<^sub>r\<^sub>u\<^sub>n \<inter> \<lbrakk>\<lbrakk> \<Psi>\<^sub>2 \<nabla> n\<^sub>2 \<rbrakk>\<rbrakk>\<^sub>T\<^sub>E\<^sub>S\<^sub>L \<inter> \<lbrakk>\<lbrakk> \<Phi>\<^sub>2 \<nabla> Suc n\<^sub>2 \<rbrakk>\<rbrakk>\<^sub>T\<^sub>E\<^sub>S\<^sub>L \<subseteq> \<lbrakk>\<lbrakk> \<Gamma>\<^sub>1 \<rbrakk>\<rbrakk>\<^sub>s\<^sub>y\<^sub>m\<^sub>r\<^sub>u\<^sub>n \<inter> \<lbrakk>\<lbrakk> \<Psi>\<^sub>1 \<nabla> n\<^sub>1 \<rbrakk>\<rbrakk>\<^sub>T\<^sub>E\<^sub>S\<^sub>L \<inter> \<lbrakk>\<lbrakk> \<Phi>\<^sub>1 \<nabla> Suc n\<^sub>1 \<rbrakk>\<rbrakk>\<^sub>T\<^sub>E\<^sub>S\<^sub>L"
-    using TESL_interp_at_index_sporadic_cases
-  proof -
-    fix K :: clock and n :: nat and \<tau> :: tag_const and \<Gamma> :: "constr list" and \<Psi> :: "TESL_atomic list" and \<Phi> :: "TESL_atomic list"
-    assume a1: "(\<Gamma>\<^sub>2, n\<^sub>2 \<turnstile> \<Psi>\<^sub>2 \<triangleright> \<Phi>\<^sub>2) = (K \<Up> n # K \<Down> n @ \<lfloor> \<tau> \<rfloor> # \<Gamma>, n \<turnstile> \<Psi> \<triangleright> \<Phi>)"
-    assume a2: "(\<Gamma>\<^sub>1, n\<^sub>1 \<turnstile> \<Psi>\<^sub>1 \<triangleright> \<Phi>\<^sub>1) = (\<Gamma>, n \<turnstile> (K sporadic \<tau>) # \<Psi> \<triangleright> \<Phi>)"
-    have f3: "\<lbrakk> K \<Up> n \<rbrakk>\<^sub>s\<^sub>y\<^sub>m\<^sub>r\<^sub>u\<^sub>n \<inter> (\<lbrakk> K \<Down> n @ \<lfloor> \<tau> \<rfloor> \<rbrakk>\<^sub>s\<^sub>y\<^sub>m\<^sub>r\<^sub>u\<^sub>n \<inter> \<lbrakk>\<lbrakk> \<Gamma> \<rbrakk>\<rbrakk>\<^sub>s\<^sub>y\<^sub>m\<^sub>r\<^sub>u\<^sub>n) = \<lbrakk>\<lbrakk> \<Gamma>\<^sub>2 \<rbrakk>\<rbrakk>\<^sub>s\<^sub>y\<^sub>m\<^sub>r\<^sub>u\<^sub>n"
-      using a1 by force
-    have "(\<lbrakk> K \<Up> n \<rbrakk>\<^sub>s\<^sub>y\<^sub>m\<^sub>r\<^sub>u\<^sub>n \<inter> \<lbrakk> K \<Down> n @ \<lfloor> \<tau> \<rfloor> \<rbrakk>\<^sub>s\<^sub>y\<^sub>m\<^sub>r\<^sub>u\<^sub>n \<union> \<lbrakk> K sporadic \<tau> \<nabla> Suc n \<rbrakk>\<^sub>T\<^sub>E\<^sub>S\<^sub>L) \<inter> \<lbrakk>\<lbrakk> \<Psi>\<^sub>2 \<nabla> n\<^sub>2 \<rbrakk>\<rbrakk>\<^sub>T\<^sub>E\<^sub>S\<^sub>L = \<lbrakk>\<lbrakk> \<Psi>\<^sub>1 \<nabla> n\<^sub>1 \<rbrakk>\<rbrakk>\<^sub>T\<^sub>E\<^sub>S\<^sub>L"
-      using a2 a1 by (metis (no_types) Pair_inject TESL_interp_at_index_sporadic_cases TESL_interpretation_at_index_cons_morph)
-    then show "\<lbrakk>\<lbrakk> \<Gamma>\<^sub>2 \<rbrakk>\<rbrakk>\<^sub>s\<^sub>y\<^sub>m\<^sub>r\<^sub>u\<^sub>n \<inter> \<lbrakk>\<lbrakk> \<Psi>\<^sub>2 \<nabla> n\<^sub>2 \<rbrakk>\<rbrakk>\<^sub>T\<^sub>E\<^sub>S\<^sub>L \<inter> \<lbrakk>\<lbrakk> \<Phi>\<^sub>2 \<nabla> Suc n\<^sub>2 \<rbrakk>\<rbrakk>\<^sub>T\<^sub>E\<^sub>S\<^sub>L \<subseteq> \<lbrakk>\<lbrakk> \<Gamma>\<^sub>1 \<rbrakk>\<rbrakk>\<^sub>s\<^sub>y\<^sub>m\<^sub>r\<^sub>u\<^sub>n \<inter> \<lbrakk>\<lbrakk> \<Psi>\<^sub>1 \<nabla> n\<^sub>1 \<rbrakk>\<rbrakk>\<^sub>T\<^sub>E\<^sub>S\<^sub>L \<inter> \<lbrakk>\<lbrakk> \<Phi>\<^sub>1 \<nabla> Suc n\<^sub>1 \<rbrakk>\<rbrakk>\<^sub>T\<^sub>E\<^sub>S\<^sub>L"
-      using f3 a2 a1 by blast
-  qed
-  show "\<And>\<Gamma> n K\<^sub>1 \<tau> K\<^sub>2 \<Psi> \<Phi>.
-       (\<Gamma>\<^sub>1, n\<^sub>1 \<turnstile> \<Psi>\<^sub>1 \<triangleright> \<Phi>\<^sub>1) = (\<Gamma>, n \<turnstile> (K\<^sub>1 sporadic \<tau> on K\<^sub>2) # \<Psi> \<triangleright> \<Phi>) \<Longrightarrow>
-       (\<Gamma>\<^sub>2, n\<^sub>2 \<turnstile> \<Psi>\<^sub>2 \<triangleright> \<Phi>\<^sub>2) = (\<Gamma>, n \<turnstile> \<Psi> \<triangleright> (K\<^sub>1 sporadic \<tau> on K\<^sub>2) # \<Phi>) \<Longrightarrow>
-       (* consistent_run \<Gamma> \<Longrightarrow> *)
-       \<lbrakk>\<lbrakk> \<Gamma>\<^sub>2 \<rbrakk>\<rbrakk>\<^sub>s\<^sub>y\<^sub>m\<^sub>r\<^sub>u\<^sub>n \<inter> \<lbrakk>\<lbrakk> \<Psi>\<^sub>2 \<nabla> n\<^sub>2 \<rbrakk>\<rbrakk>\<^sub>T\<^sub>E\<^sub>S\<^sub>L \<inter> \<lbrakk>\<lbrakk> \<Phi>\<^sub>2 \<nabla> Suc n\<^sub>2 \<rbrakk>\<rbrakk>\<^sub>T\<^sub>E\<^sub>S\<^sub>L \<subseteq> \<lbrakk>\<lbrakk> \<Gamma>\<^sub>1 \<rbrakk>\<rbrakk>\<^sub>s\<^sub>y\<^sub>m\<^sub>r\<^sub>u\<^sub>n \<inter> \<lbrakk>\<lbrakk> \<Psi>\<^sub>1 \<nabla> n\<^sub>1 \<rbrakk>\<rbrakk>\<^sub>T\<^sub>E\<^sub>S\<^sub>L \<inter> \<lbrakk>\<lbrakk> \<Phi>\<^sub>1 \<nabla> Suc n\<^sub>1 \<rbrakk>\<rbrakk>\<^sub>T\<^sub>E\<^sub>S\<^sub>L"
-    using TESL_interp_at_index_sporadicon_cases
-    proof -
-    fix \<Gamma> :: "constr list" and n :: nat and K\<^sub>1 :: clock and \<tau> :: tag_expr and K\<^sub>2 :: clock and \<Psi> :: "TESL_atomic list" and \<Phi> :: "TESL_atomic list"
-    assume a1: "(\<Gamma>\<^sub>1, n\<^sub>1 \<turnstile> \<Psi>\<^sub>1 \<triangleright> \<Phi>\<^sub>1) = (\<Gamma>, n \<turnstile> (K\<^sub>1 sporadic \<tau> on K\<^sub>2) # \<Psi> \<triangleright> \<Phi>)"
-    assume a2: "(\<Gamma>\<^sub>2, n\<^sub>2 \<turnstile> \<Psi>\<^sub>2 \<triangleright> \<Phi>\<^sub>2) = (\<Gamma>, n \<turnstile> \<Psi> \<triangleright> (K\<^sub>1 sporadic \<tau> on K\<^sub>2) # \<Phi>)"
-    have "n\<^sub>1 = n \<and> (\<Psi>\<^sub>1, \<Phi>\<^sub>1) = ((K\<^sub>1 sporadic \<tau> on K\<^sub>2) # \<Psi>, \<Phi>)"
-      using a1 by fastforce
-    then have f3: "\<lbrakk> K\<^sub>1 sporadic \<tau> on K\<^sub>2 \<nabla> Suc n\<^sub>1 \<rbrakk>\<^sub>T\<^sub>E\<^sub>S\<^sub>L \<subseteq> \<lbrakk> K\<^sub>1 sporadic \<tau> on K\<^sub>2 \<nabla> n \<rbrakk>\<^sub>T\<^sub>E\<^sub>S\<^sub>L"
-      using TESL_interp_at_index_sporadicon_cases by blast
-    have f4: "\<lbrakk> K\<^sub>1 sporadic \<tau> on K\<^sub>2 \<nabla> Suc n\<^sub>1 \<rbrakk>\<^sub>T\<^sub>E\<^sub>S\<^sub>L \<inter> \<lbrakk>\<lbrakk> \<Phi>\<^sub>1 \<nabla> Suc n\<^sub>1 \<rbrakk>\<rbrakk>\<^sub>T\<^sub>E\<^sub>S\<^sub>L = \<lbrakk>\<lbrakk> \<Phi>\<^sub>2 \<nabla> Suc n\<^sub>2 \<rbrakk>\<rbrakk>\<^sub>T\<^sub>E\<^sub>S\<^sub>L"
-      using a2 a1 by force
-    have "\<lbrakk> K\<^sub>1 sporadic \<tau> on K\<^sub>2 \<nabla> n \<rbrakk>\<^sub>T\<^sub>E\<^sub>S\<^sub>L \<inter> \<lbrakk>\<lbrakk> \<Psi>\<^sub>2 \<nabla> n\<^sub>2 \<rbrakk>\<rbrakk>\<^sub>T\<^sub>E\<^sub>S\<^sub>L = \<lbrakk>\<lbrakk> \<Psi>\<^sub>1 \<nabla> n\<^sub>1 \<rbrakk>\<rbrakk>\<^sub>T\<^sub>E\<^sub>S\<^sub>L"
-      using a2 a1 by force
-    then show "\<lbrakk>\<lbrakk> \<Gamma>\<^sub>2 \<rbrakk>\<rbrakk>\<^sub>s\<^sub>y\<^sub>m\<^sub>r\<^sub>u\<^sub>n \<inter> \<lbrakk>\<lbrakk> \<Psi>\<^sub>2 \<nabla> n\<^sub>2 \<rbrakk>\<rbrakk>\<^sub>T\<^sub>E\<^sub>S\<^sub>L \<inter> \<lbrakk>\<lbrakk> \<Phi>\<^sub>2 \<nabla> Suc n\<^sub>2 \<rbrakk>\<rbrakk>\<^sub>T\<^sub>E\<^sub>S\<^sub>L \<subseteq> \<lbrakk>\<lbrakk> \<Gamma>\<^sub>1 \<rbrakk>\<rbrakk>\<^sub>s\<^sub>y\<^sub>m\<^sub>r\<^sub>u\<^sub>n \<inter> \<lbrakk>\<lbrakk> \<Psi>\<^sub>1 \<nabla> n\<^sub>1 \<rbrakk>\<rbrakk>\<^sub>T\<^sub>E\<^sub>S\<^sub>L \<inter> \<lbrakk>\<lbrakk> \<Phi>\<^sub>1 \<nabla> Suc n\<^sub>1 \<rbrakk>\<rbrakk>\<^sub>T\<^sub>E\<^sub>S\<^sub>L"
-      using f4 f3 a2 a1 by blast
-  qed
-  show "\<And>K\<^sub>1 n K\<^sub>2 \<tau> \<Gamma> \<Psi> \<Phi>.
-       (\<Gamma>\<^sub>1, n\<^sub>1 \<turnstile> \<Psi>\<^sub>1 \<triangleright> \<Phi>\<^sub>1) = (\<Gamma>, n \<turnstile> (K\<^sub>1 sporadic \<tau> on K\<^sub>2) # \<Psi> \<triangleright> \<Phi>) \<Longrightarrow>
-       (\<Gamma>\<^sub>2, n\<^sub>2 \<turnstile> \<Psi>\<^sub>2 \<triangleright> \<Phi>\<^sub>2) = (K\<^sub>1 \<Up> n # K\<^sub>2 \<Down> n @ \<tau> # \<Gamma>, n \<turnstile> \<Psi> \<triangleright> \<Phi>) \<Longrightarrow>
-       (* consistent_run (K\<^sub>1 \<Up> n # K\<^sub>2 \<Down> n @ \<tau> # \<Gamma>) \<Longrightarrow> *)
-       \<lbrakk>\<lbrakk> \<Gamma>\<^sub>2 \<rbrakk>\<rbrakk>\<^sub>s\<^sub>y\<^sub>m\<^sub>r\<^sub>u\<^sub>n \<inter> \<lbrakk>\<lbrakk> \<Psi>\<^sub>2 \<nabla> n\<^sub>2 \<rbrakk>\<rbrakk>\<^sub>T\<^sub>E\<^sub>S\<^sub>L \<inter> \<lbrakk>\<lbrakk> \<Phi>\<^sub>2 \<nabla> Suc n\<^sub>2 \<rbrakk>\<rbrakk>\<^sub>T\<^sub>E\<^sub>S\<^sub>L \<subseteq> \<lbrakk>\<lbrakk> \<Gamma>\<^sub>1 \<rbrakk>\<rbrakk>\<^sub>s\<^sub>y\<^sub>m\<^sub>r\<^sub>u\<^sub>n \<inter> \<lbrakk>\<lbrakk> \<Psi>\<^sub>1 \<nabla> n\<^sub>1 \<rbrakk>\<rbrakk>\<^sub>T\<^sub>E\<^sub>S\<^sub>L \<inter> \<lbrakk>\<lbrakk> \<Phi>\<^sub>1 \<nabla> Suc n\<^sub>1 \<rbrakk>\<rbrakk>\<^sub>T\<^sub>E\<^sub>S\<^sub>L"
-    using TESL_interp_at_index_sporadicon_cases
-    proof -
-    fix K\<^sub>1 :: clock and n :: nat and K\<^sub>2 :: clock and \<tau> :: tag_expr and \<Gamma> :: "constr list" and \<Psi> :: "TESL_atomic list" and \<Phi> :: "TESL_atomic list"
-    assume a1: "(\<Gamma>\<^sub>1, n\<^sub>1 \<turnstile> \<Psi>\<^sub>1 \<triangleright> \<Phi>\<^sub>1) = (\<Gamma>, n \<turnstile> (K\<^sub>1 sporadic \<tau> on K\<^sub>2) # \<Psi> \<triangleright> \<Phi>)"
-    assume a2: "(\<Gamma>\<^sub>2, n\<^sub>2 \<turnstile> \<Psi>\<^sub>2 \<triangleright> \<Phi>\<^sub>2) = (K\<^sub>1 \<Up> n # K\<^sub>2 \<Down> n @ \<tau> # \<Gamma>, n \<turnstile> \<Psi> \<triangleright> \<Phi>)"
-    then have f3: "\<lbrakk>\<lbrakk> \<Gamma>\<^sub>1 \<rbrakk>\<rbrakk>\<^sub>s\<^sub>y\<^sub>m\<^sub>r\<^sub>u\<^sub>n \<inter> (\<lbrakk>\<lbrakk> \<Gamma>\<^sub>2 \<rbrakk>\<rbrakk>\<^sub>s\<^sub>y\<^sub>m\<^sub>r\<^sub>u\<^sub>n \<inter> (\<lbrakk>\<lbrakk> \<Psi>\<^sub>2 \<nabla> n\<^sub>2 \<rbrakk>\<rbrakk>\<^sub>T\<^sub>E\<^sub>S\<^sub>L \<inter> \<lbrakk>\<lbrakk> \<Phi>\<^sub>2 \<nabla> Suc n\<^sub>2 \<rbrakk>\<rbrakk>\<^sub>T\<^sub>E\<^sub>S\<^sub>L)) \<subseteq> (\<Inter>t\<in>set \<Psi>\<^sub>2. \<lbrakk> t \<nabla> n\<^sub>2 \<rbrakk>\<^sub>T\<^sub>E\<^sub>S\<^sub>L) \<inter> (\<lbrakk>\<lbrakk> \<Gamma>\<^sub>1 \<rbrakk>\<rbrakk>\<^sub>s\<^sub>y\<^sub>m\<^sub>r\<^sub>u\<^sub>n \<inter> (\<Inter>t\<in>set \<Phi>\<^sub>1. \<lbrakk> t \<nabla> Suc n\<^sub>1 \<rbrakk>\<^sub>T\<^sub>E\<^sub>S\<^sub>L))"
-    using a1 TESL_interpretation_at_index_fixpoint by force
-    have f4: "\<lbrakk> K\<^sub>1 \<Up> n \<rbrakk>\<^sub>s\<^sub>y\<^sub>m\<^sub>r\<^sub>u\<^sub>n \<inter> (\<lbrakk> K\<^sub>2 \<Down> n @ \<tau> \<rbrakk>\<^sub>s\<^sub>y\<^sub>m\<^sub>r\<^sub>u\<^sub>n \<inter> \<lbrakk> K\<^sub>2 \<Down> n @ \<tau> \<rbrakk>\<^sub>s\<^sub>y\<^sub>m\<^sub>r\<^sub>u\<^sub>n) \<inter> (\<lbrakk>\<lbrakk> \<Gamma>\<^sub>1 \<rbrakk>\<rbrakk>\<^sub>s\<^sub>y\<^sub>m\<^sub>r\<^sub>u\<^sub>n \<inter> (\<lbrakk>\<lbrakk> \<Gamma>\<^sub>2 \<rbrakk>\<rbrakk>\<^sub>s\<^sub>y\<^sub>m\<^sub>r\<^sub>u\<^sub>n \<inter> (\<lbrakk>\<lbrakk> \<Psi>\<^sub>2 \<nabla> n\<^sub>2 \<rbrakk>\<rbrakk>\<^sub>T\<^sub>E\<^sub>S\<^sub>L \<inter> \<lbrakk>\<lbrakk> \<Phi>\<^sub>2 \<nabla> Suc n\<^sub>2 \<rbrakk>\<rbrakk>\<^sub>T\<^sub>E\<^sub>S\<^sub>L))) = \<lbrakk>\<lbrakk> \<Gamma>\<^sub>2 \<rbrakk>\<rbrakk>\<^sub>s\<^sub>y\<^sub>m\<^sub>r\<^sub>u\<^sub>n \<inter> (\<lbrakk>\<lbrakk> \<Psi>\<^sub>2 \<nabla> n\<^sub>2 \<rbrakk>\<rbrakk>\<^sub>T\<^sub>E\<^sub>S\<^sub>L \<inter> \<lbrakk>\<lbrakk> \<Phi>\<^sub>2 \<nabla> Suc n\<^sub>2 \<rbrakk>\<rbrakk>\<^sub>T\<^sub>E\<^sub>S\<^sub>L)"
-      using a2 a1 by force
-    have "\<lbrakk> K\<^sub>1 sporadic \<tau> on K\<^sub>2 \<nabla> n \<rbrakk>\<^sub>T\<^sub>E\<^sub>S\<^sub>L \<inter> (\<Inter>t\<in>set \<Psi>\<^sub>2. \<lbrakk> t \<nabla> n\<^sub>2 \<rbrakk>\<^sub>T\<^sub>E\<^sub>S\<^sub>L) \<inter> (\<lbrakk>\<lbrakk> \<Gamma>\<^sub>1 \<rbrakk>\<rbrakk>\<^sub>s\<^sub>y\<^sub>m\<^sub>r\<^sub>u\<^sub>n \<inter> (\<Inter>t\<in>set \<Phi>\<^sub>1. \<lbrakk> t \<nabla> Suc n\<^sub>1 \<rbrakk>\<^sub>T\<^sub>E\<^sub>S\<^sub>L)) = (\<Inter>t\<in>set \<Psi>\<^sub>1. \<lbrakk> t \<nabla> n\<^sub>1 \<rbrakk>\<^sub>T\<^sub>E\<^sub>S\<^sub>L) \<inter> (\<lbrakk>\<lbrakk> \<Gamma>\<^sub>1 \<rbrakk>\<rbrakk>\<^sub>s\<^sub>y\<^sub>m\<^sub>r\<^sub>u\<^sub>n \<inter> (\<lbrakk>\<lbrakk> \<Gamma>\<^sub>1 \<rbrakk>\<rbrakk>\<^sub>s\<^sub>y\<^sub>m\<^sub>r\<^sub>u\<^sub>n \<inter> (\<Inter>t\<in>set \<Phi>\<^sub>1. \<lbrakk> t \<nabla> Suc n\<^sub>1 \<rbrakk>\<^sub>T\<^sub>E\<^sub>S\<^sub>L)))"
-      using a2 a1 by simp
-    then have "(\<lbrakk> K\<^sub>1 \<Up> n \<rbrakk>\<^sub>s\<^sub>y\<^sub>m\<^sub>r\<^sub>u\<^sub>n \<inter> \<lbrakk> K\<^sub>2 \<Down> n @ \<tau> \<rbrakk>\<^sub>s\<^sub>y\<^sub>m\<^sub>r\<^sub>u\<^sub>n \<union> \<lbrakk> K\<^sub>1 sporadic \<tau> on K\<^sub>2 \<nabla> Suc n \<rbrakk>\<^sub>T\<^sub>E\<^sub>S\<^sub>L) \<inter> ((\<Inter>t\<in>set \<Psi>\<^sub>2. \<lbrakk> t \<nabla> n\<^sub>2 \<rbrakk>\<^sub>T\<^sub>E\<^sub>S\<^sub>L) \<inter> (\<lbrakk>\<lbrakk> \<Gamma>\<^sub>1 \<rbrakk>\<rbrakk>\<^sub>s\<^sub>y\<^sub>m\<^sub>r\<^sub>u\<^sub>n \<inter> (\<Inter>t\<in>set \<Phi>\<^sub>1. \<lbrakk> t \<nabla> Suc n\<^sub>1 \<rbrakk>\<^sub>T\<^sub>E\<^sub>S\<^sub>L))) = \<lbrakk>\<lbrakk> \<Gamma>\<^sub>1 \<rbrakk>\<rbrakk>\<^sub>s\<^sub>y\<^sub>m\<^sub>r\<^sub>u\<^sub>n \<inter> (\<lbrakk>\<lbrakk> \<Psi>\<^sub>1 \<nabla> n\<^sub>1 \<rbrakk>\<rbrakk>\<^sub>T\<^sub>E\<^sub>S\<^sub>L \<inter> \<lbrakk>\<lbrakk> \<Phi>\<^sub>1 \<nabla> Suc n\<^sub>1 \<rbrakk>\<rbrakk>\<^sub>T\<^sub>E\<^sub>S\<^sub>L)"
-      by (metis Int_absorb TESL_interp_at_index_sporadicon_cases TESL_interpretation_at_index_fixpoint inf_aci(2) inf_left_commute)
-    then show "\<lbrakk>\<lbrakk> \<Gamma>\<^sub>2 \<rbrakk>\<rbrakk>\<^sub>s\<^sub>y\<^sub>m\<^sub>r\<^sub>u\<^sub>n \<inter> \<lbrakk>\<lbrakk> \<Psi>\<^sub>2 \<nabla> n\<^sub>2 \<rbrakk>\<rbrakk>\<^sub>T\<^sub>E\<^sub>S\<^sub>L \<inter> \<lbrakk>\<lbrakk> \<Phi>\<^sub>2 \<nabla> Suc n\<^sub>2 \<rbrakk>\<rbrakk>\<^sub>T\<^sub>E\<^sub>S\<^sub>L \<subseteq> \<lbrakk>\<lbrakk> \<Gamma>\<^sub>1 \<rbrakk>\<rbrakk>\<^sub>s\<^sub>y\<^sub>m\<^sub>r\<^sub>u\<^sub>n \<inter> \<lbrakk>\<lbrakk> \<Psi>\<^sub>1 \<nabla> n\<^sub>1 \<rbrakk>\<rbrakk>\<^sub>T\<^sub>E\<^sub>S\<^sub>L \<inter> \<lbrakk>\<lbrakk> \<Phi>\<^sub>1 \<nabla> Suc n\<^sub>1 \<rbrakk>\<rbrakk>\<^sub>T\<^sub>E\<^sub>S\<^sub>L"
-      using f4 f3 by blast
-  qed
-  show "\<And>K\<^sub>1 n \<alpha> K\<^sub>2 \<beta> \<Gamma> \<Psi> \<Phi>.
-       (\<Gamma>\<^sub>1, n\<^sub>1 \<turnstile> \<Psi>\<^sub>1 \<triangleright> \<Phi>\<^sub>1) = (\<Gamma>, n \<turnstile> (tag-relation K\<^sub>1 = \<alpha> * K\<^sub>2 + \<beta>) # \<Psi> \<triangleright> \<Phi>) \<Longrightarrow>
-       (\<Gamma>\<^sub>2, n\<^sub>2 \<turnstile> \<Psi>\<^sub>2 \<triangleright> \<Phi>\<^sub>2) = (\<tau>\<^sub>v\<^sub>a\<^sub>r (K\<^sub>1, n) \<doteq> \<alpha> * \<tau>\<^sub>v\<^sub>a\<^sub>r (K\<^sub>2, n) + \<beta> # \<Gamma>, n \<turnstile> \<Psi> \<triangleright> (tag-relation K\<^sub>1 = \<alpha> * K\<^sub>2 + \<beta>) # \<Phi>) \<Longrightarrow>
-       (* consistent_run (\<tau>\<^sub>v\<^sub>a\<^sub>r (K\<^sub>1, n) \<doteq> \<alpha> * \<tau>\<^sub>v\<^sub>a\<^sub>r (K\<^sub>2, n) + \<beta> # \<Gamma>) \<Longrightarrow> *)
-       \<lbrakk>\<lbrakk> \<Gamma>\<^sub>2 \<rbrakk>\<rbrakk>\<^sub>s\<^sub>y\<^sub>m\<^sub>r\<^sub>u\<^sub>n \<inter> \<lbrakk>\<lbrakk> \<Psi>\<^sub>2 \<nabla> n\<^sub>2 \<rbrakk>\<rbrakk>\<^sub>T\<^sub>E\<^sub>S\<^sub>L \<inter> \<lbrakk>\<lbrakk> \<Phi>\<^sub>2 \<nabla> Suc n\<^sub>2 \<rbrakk>\<rbrakk>\<^sub>T\<^sub>E\<^sub>S\<^sub>L \<subseteq> \<lbrakk>\<lbrakk> \<Gamma>\<^sub>1 \<rbrakk>\<rbrakk>\<^sub>s\<^sub>y\<^sub>m\<^sub>r\<^sub>u\<^sub>n \<inter> \<lbrakk>\<lbrakk> \<Psi>\<^sub>1 \<nabla> n\<^sub>1 \<rbrakk>\<rbrakk>\<^sub>T\<^sub>E\<^sub>S\<^sub>L \<inter> \<lbrakk>\<lbrakk> \<Phi>\<^sub>1 \<nabla> Suc n\<^sub>1 \<rbrakk>\<rbrakk>\<^sub>T\<^sub>E\<^sub>S\<^sub>L"
-    using TESL_interp_at_index_tagrel_cases
-    proof -
-      fix K\<^sub>1 :: clock and n :: nat and \<alpha> :: tag_const and K\<^sub>2 :: clock and \<beta> :: tag_const and \<Gamma> :: "constr list" and \<Psi> :: "TESL_atomic list" and \<Phi> :: "TESL_atomic list"
-    assume a1: "(\<Gamma>\<^sub>2, n\<^sub>2 \<turnstile> \<Psi>\<^sub>2 \<triangleright> \<Phi>\<^sub>2) = (\<tau>\<^sub>v\<^sub>a\<^sub>r (K\<^sub>1, n) \<doteq> \<alpha> * \<tau>\<^sub>v\<^sub>a\<^sub>r (K\<^sub>2, n) + \<beta> # \<Gamma>, n \<turnstile> \<Psi> \<triangleright> (tag-relation K\<^sub>1 = \<alpha> * K\<^sub>2 + \<beta>) # \<Phi>)"
-    assume a2: "(\<Gamma>\<^sub>1, n\<^sub>1 \<turnstile> \<Psi>\<^sub>1 \<triangleright> \<Phi>\<^sub>1) = (\<Gamma>, n \<turnstile> (tag-relation K\<^sub>1 = \<alpha> * K\<^sub>2 + \<beta>) # \<Psi> \<triangleright> \<Phi>)"
-    have f3: "\<forall>ts tsa tsb tsc. (ts::TESL_atomic list, tsa::TESL_atomic list) \<noteq> (tsb, tsc) \<or> ts = tsb \<and> tsa = tsc"
-      by fastforce
-    have f4: "n\<^sub>2 = n \<and> (\<Psi>\<^sub>2, \<Phi>\<^sub>2) = (\<Psi>, (tag-relation K\<^sub>1 = \<alpha> * K\<^sub>2 + \<beta>) # \<Phi>)"
-      using a1 by fastforce
-    have f5: "\<lbrakk>\<lbrakk> (tag-relation K\<^sub>1 = \<alpha> * K\<^sub>2 + \<beta>) # \<Phi> \<nabla> Suc n \<rbrakk>\<rbrakk>\<^sub>T\<^sub>E\<^sub>S\<^sub>L = \<lbrakk>\<lbrakk> \<Phi>\<^sub>2 \<nabla> Suc n\<^sub>2 \<rbrakk>\<rbrakk>\<^sub>T\<^sub>E\<^sub>S\<^sub>L"
-      using a1 by force
-    have f6: "n\<^sub>1 = n \<and> (\<Psi>\<^sub>1, \<Phi>\<^sub>1) = ((tag-relation K\<^sub>1 = \<alpha> * K\<^sub>2 + \<beta>) # \<Psi>, \<Phi>)"
-      using a2 by fastforce
-    have f7: "\<lbrakk>\<lbrakk> \<Phi> \<nabla> Suc n \<rbrakk>\<rbrakk>\<^sub>T\<^sub>E\<^sub>S\<^sub>L = \<lbrakk>\<lbrakk> \<Phi>\<^sub>1 \<nabla> Suc n\<^sub>1 \<rbrakk>\<rbrakk>\<^sub>T\<^sub>E\<^sub>S\<^sub>L"
-      using a2 by force
-    have f8: "\<lbrakk>\<lbrakk> \<tau>\<^sub>v\<^sub>a\<^sub>r (K\<^sub>1, n) \<doteq> \<alpha> * \<tau>\<^sub>v\<^sub>a\<^sub>r (K\<^sub>2, n) + \<beta> # \<Gamma> \<rbrakk>\<rbrakk>\<^sub>s\<^sub>y\<^sub>m\<^sub>r\<^sub>u\<^sub>n = \<lbrakk> \<tau>\<^sub>v\<^sub>a\<^sub>r (K\<^sub>1, n) \<doteq> \<alpha> * \<tau>\<^sub>v\<^sub>a\<^sub>r (K\<^sub>2, n) + \<beta> \<rbrakk>\<^sub>s\<^sub>y\<^sub>m\<^sub>r\<^sub>u\<^sub>n \<inter> \<lbrakk>\<lbrakk> \<Gamma>\<^sub>1 \<rbrakk>\<rbrakk>\<^sub>s\<^sub>y\<^sub>m\<^sub>r\<^sub>u\<^sub>n"
-      using a2 by force
-    have f9: "\<lbrakk> tag-relation K\<^sub>1 = \<alpha> * K\<^sub>2 + \<beta> \<nabla> Suc n \<rbrakk>\<^sub>T\<^sub>E\<^sub>S\<^sub>L \<inter> (\<lbrakk>\<lbrakk> \<Psi>\<^sub>2 \<nabla> n\<^sub>2 \<rbrakk>\<rbrakk>\<^sub>T\<^sub>E\<^sub>S\<^sub>L \<inter> \<lbrakk> \<tau>\<^sub>v\<^sub>a\<^sub>r (K\<^sub>1, n) \<doteq> \<alpha> * \<tau>\<^sub>v\<^sub>a\<^sub>r (K\<^sub>2, n) + \<beta> \<rbrakk>\<^sub>s\<^sub>y\<^sub>m\<^sub>r\<^sub>u\<^sub>n) = \<lbrakk>\<lbrakk> \<Psi>\<^sub>1 \<nabla> n\<^sub>1 \<rbrakk>\<rbrakk>\<^sub>T\<^sub>E\<^sub>S\<^sub>L"
-      using f6 f4 f3 by (metis Int_commute TESL_interp_at_index_tagrel_cases TESL_interpretation_at_index_cons_morph inf_sup_aci(3))
-    have "\<lbrakk> tag-relation K\<^sub>1 = \<alpha> * K\<^sub>2 + \<beta> \<nabla> Suc n \<rbrakk>\<^sub>T\<^sub>E\<^sub>S\<^sub>L \<inter> \<lbrakk>\<lbrakk> \<Phi>\<^sub>1 \<nabla> Suc n\<^sub>1 \<rbrakk>\<rbrakk>\<^sub>T\<^sub>E\<^sub>S\<^sub>L = \<lbrakk>\<lbrakk> \<Phi>\<^sub>2 \<nabla> Suc n\<^sub>2 \<rbrakk>\<rbrakk>\<^sub>T\<^sub>E\<^sub>S\<^sub>L"
-      using f7 f5 by simp
-    then show "\<lbrakk>\<lbrakk> \<Gamma>\<^sub>2 \<rbrakk>\<rbrakk>\<^sub>s\<^sub>y\<^sub>m\<^sub>r\<^sub>u\<^sub>n \<inter> \<lbrakk>\<lbrakk> \<Psi>\<^sub>2 \<nabla> n\<^sub>2 \<rbrakk>\<rbrakk>\<^sub>T\<^sub>E\<^sub>S\<^sub>L \<inter> \<lbrakk>\<lbrakk> \<Phi>\<^sub>2 \<nabla> Suc n\<^sub>2 \<rbrakk>\<rbrakk>\<^sub>T\<^sub>E\<^sub>S\<^sub>L \<subseteq> \<lbrakk>\<lbrakk> \<Gamma>\<^sub>1 \<rbrakk>\<rbrakk>\<^sub>s\<^sub>y\<^sub>m\<^sub>r\<^sub>u\<^sub>n \<inter> \<lbrakk>\<lbrakk> \<Psi>\<^sub>1 \<nabla> n\<^sub>1 \<rbrakk>\<rbrakk>\<^sub>T\<^sub>E\<^sub>S\<^sub>L \<inter> \<lbrakk>\<lbrakk> \<Phi>\<^sub>1 \<nabla> Suc n\<^sub>1 \<rbrakk>\<rbrakk>\<^sub>T\<^sub>E\<^sub>S\<^sub>L"
-      using f9 f8 a1 by blast
-  qed
-  show "\<And>K\<^sub>1 n \<Gamma> K\<^sub>2 \<Psi> \<Phi>.
-       (\<Gamma>\<^sub>1, n\<^sub>1 \<turnstile> \<Psi>\<^sub>1 \<triangleright> \<Phi>\<^sub>1) = (\<Gamma>, n \<turnstile> (K\<^sub>1 implies K\<^sub>2) # \<Psi> \<triangleright> \<Phi>) \<Longrightarrow>
-       (\<Gamma>\<^sub>2, n\<^sub>2 \<turnstile> \<Psi>\<^sub>2 \<triangleright> \<Phi>\<^sub>2) = (K\<^sub>1 \<not>\<Up> n # \<Gamma>, n \<turnstile> \<Psi> \<triangleright> (K\<^sub>1 implies K\<^sub>2) # \<Phi>) \<Longrightarrow>
-       (* consistent_run (K\<^sub>1 \<not>\<Up> n # \<Gamma>) \<Longrightarrow> *)
-       \<lbrakk>\<lbrakk> \<Gamma>\<^sub>2 \<rbrakk>\<rbrakk>\<^sub>s\<^sub>y\<^sub>m\<^sub>r\<^sub>u\<^sub>n \<inter> \<lbrakk>\<lbrakk> \<Psi>\<^sub>2 \<nabla> n\<^sub>2 \<rbrakk>\<rbrakk>\<^sub>T\<^sub>E\<^sub>S\<^sub>L \<inter> \<lbrakk>\<lbrakk> \<Phi>\<^sub>2 \<nabla> Suc n\<^sub>2 \<rbrakk>\<rbrakk>\<^sub>T\<^sub>E\<^sub>S\<^sub>L \<subseteq> \<lbrakk>\<lbrakk> \<Gamma>\<^sub>1 \<rbrakk>\<rbrakk>\<^sub>s\<^sub>y\<^sub>m\<^sub>r\<^sub>u\<^sub>n \<inter> \<lbrakk>\<lbrakk> \<Psi>\<^sub>1 \<nabla> n\<^sub>1 \<rbrakk>\<rbrakk>\<^sub>T\<^sub>E\<^sub>S\<^sub>L \<inter> \<lbrakk>\<lbrakk> \<Phi>\<^sub>1 \<nabla> Suc n\<^sub>1 \<rbrakk>\<rbrakk>\<^sub>T\<^sub>E\<^sub>S\<^sub>L"
-    using TESL_interp_at_index_implies_cases
-    using [[smt_solver = cvc4]]
-    by (smt Int_subset_iff Pair_inject TESL_interpretation_at_index.elims inf.cobounded2 inf.mono inf_sup_aci(2) list.simps(1) list.simps(3) sup.cobounded1 symbolic_run_interpretation.simps(2))
-  show "\<And>K\<^sub>1 n K\<^sub>2 \<Gamma> \<Psi> \<Phi>.
-       (\<Gamma>\<^sub>1, n\<^sub>1 \<turnstile> \<Psi>\<^sub>1 \<triangleright> \<Phi>\<^sub>1) = (\<Gamma>, n \<turnstile> (K\<^sub>1 implies K\<^sub>2) # \<Psi> \<triangleright> \<Phi>) \<Longrightarrow>
-       (\<Gamma>\<^sub>2, n\<^sub>2 \<turnstile> \<Psi>\<^sub>2 \<triangleright> \<Phi>\<^sub>2) = (K\<^sub>1 \<Up> n # K\<^sub>2 \<Up> n # \<Gamma>, n \<turnstile> \<Psi> \<triangleright> (K\<^sub>1 implies K\<^sub>2) # \<Phi>) \<Longrightarrow>
-       (* consistent_run (K\<^sub>1 \<Up> n # K\<^sub>2 \<Up> n # \<Gamma>) \<Longrightarrow> *)
-       \<lbrakk>\<lbrakk> \<Gamma>\<^sub>2 \<rbrakk>\<rbrakk>\<^sub>s\<^sub>y\<^sub>m\<^sub>r\<^sub>u\<^sub>n \<inter> \<lbrakk>\<lbrakk> \<Psi>\<^sub>2 \<nabla> n\<^sub>2 \<rbrakk>\<rbrakk>\<^sub>T\<^sub>E\<^sub>S\<^sub>L \<inter> \<lbrakk>\<lbrakk> \<Phi>\<^sub>2 \<nabla> Suc n\<^sub>2 \<rbrakk>\<rbrakk>\<^sub>T\<^sub>E\<^sub>S\<^sub>L \<subseteq> \<lbrakk>\<lbrakk> \<Gamma>\<^sub>1 \<rbrakk>\<rbrakk>\<^sub>s\<^sub>y\<^sub>m\<^sub>r\<^sub>u\<^sub>n \<inter> \<lbrakk>\<lbrakk> \<Psi>\<^sub>1 \<nabla> n\<^sub>1 \<rbrakk>\<rbrakk>\<^sub>T\<^sub>E\<^sub>S\<^sub>L \<inter> \<lbrakk>\<lbrakk> \<Phi>\<^sub>1 \<nabla> Suc n\<^sub>1 \<rbrakk>\<rbrakk>\<^sub>T\<^sub>E\<^sub>S\<^sub>L"
-    using TESL_interp_at_index_implies_cases
-    using [[smt_solver = cvc4]]
-    by (smt Int_subset_iff Pair_inject TESL_interpretation_at_index_cons_morph inf_le1 inf_sup_aci(2) le_iff_inf sup.cobounded2 symbolic_run_interpretation.simps(2))
-  show "\<And>K\<^sub>1 n \<Gamma> \<delta>\<tau> K\<^sub>2 K\<^sub>3 \<Psi> \<Phi>.
-       (\<Gamma>\<^sub>1, n\<^sub>1 \<turnstile> \<Psi>\<^sub>1 \<triangleright> \<Phi>\<^sub>1) = (\<Gamma>, n \<turnstile> (K\<^sub>1 time-delayed by \<delta>\<tau> on K\<^sub>2 implies K\<^sub>3) # \<Psi> \<triangleright> \<Phi>) \<Longrightarrow>
-       (\<Gamma>\<^sub>2, n\<^sub>2 \<turnstile> \<Psi>\<^sub>2 \<triangleright> \<Phi>\<^sub>2) = (K\<^sub>1 \<not>\<Up> n # \<Gamma>, n \<turnstile> \<Psi> \<triangleright> (K\<^sub>1 time-delayed by \<delta>\<tau> on K\<^sub>2 implies K\<^sub>3) # \<Phi>) \<Longrightarrow>
-       (* consistent_run (K\<^sub>1 \<not>\<Up> n # \<Gamma>) \<Longrightarrow> *)
-       \<lbrakk>\<lbrakk> \<Gamma>\<^sub>2 \<rbrakk>\<rbrakk>\<^sub>s\<^sub>y\<^sub>m\<^sub>r\<^sub>u\<^sub>n \<inter> \<lbrakk>\<lbrakk> \<Psi>\<^sub>2 \<nabla> n\<^sub>2 \<rbrakk>\<rbrakk>\<^sub>T\<^sub>E\<^sub>S\<^sub>L \<inter> \<lbrakk>\<lbrakk> \<Phi>\<^sub>2 \<nabla> Suc n\<^sub>2 \<rbrakk>\<rbrakk>\<^sub>T\<^sub>E\<^sub>S\<^sub>L \<subseteq> \<lbrakk>\<lbrakk> \<Gamma>\<^sub>1 \<rbrakk>\<rbrakk>\<^sub>s\<^sub>y\<^sub>m\<^sub>r\<^sub>u\<^sub>n \<inter> \<lbrakk>\<lbrakk> \<Psi>\<^sub>1 \<nabla> n\<^sub>1 \<rbrakk>\<rbrakk>\<^sub>T\<^sub>E\<^sub>S\<^sub>L \<inter> \<lbrakk>\<lbrakk> \<Phi>\<^sub>1 \<nabla> Suc n\<^sub>1 \<rbrakk>\<rbrakk>\<^sub>T\<^sub>E\<^sub>S\<^sub>L"
-    using TESL_interp_at_index_timedelayed_cases
-    using [[smt_solver = cvc4]]
-    by (smt Int_subset_iff Pair_inject TESL_interpretation_at_index_cons_morph inf.cobounded2 inf_le1 subset_trans sup.cobounded1 symbolic_run_interpretation.simps(2))
-  show "\<And>K\<^sub>1 n \<Gamma> \<delta>\<tau> K\<^sub>2 K\<^sub>3 \<Psi> \<Phi>.
-       (\<Gamma>\<^sub>1, n\<^sub>1 \<turnstile> \<Psi>\<^sub>1 \<triangleright> \<Phi>\<^sub>1) = (\<Gamma>, n \<turnstile> (K\<^sub>1 time-delayed by \<delta>\<tau> on K\<^sub>2 implies K\<^sub>3) # \<Psi> \<triangleright> \<Phi>) \<Longrightarrow>
-       (\<Gamma>\<^sub>2, n\<^sub>2 \<turnstile> \<Psi>\<^sub>2 \<triangleright> \<Phi>\<^sub>2) = (K\<^sub>1 \<Up> n # \<Gamma>, n \<turnstile> (K\<^sub>3 sporadic \<lfloor> \<tau>\<^sub>v\<^sub>a\<^sub>r (K\<^sub>2, n) \<oplus> \<delta>\<tau> \<rfloor> on K\<^sub>2) # \<Psi> \<triangleright> (K\<^sub>1 time-delayed by \<delta>\<tau> on K\<^sub>2 implies K\<^sub>3) # \<Phi>) \<Longrightarrow>
-       (* consistent_run (K\<^sub>1 \<Up> n # \<Gamma>) \<Longrightarrow> *)
-       \<lbrakk>\<lbrakk> \<Gamma>\<^sub>2 \<rbrakk>\<rbrakk>\<^sub>s\<^sub>y\<^sub>m\<^sub>r\<^sub>u\<^sub>n \<inter> \<lbrakk>\<lbrakk> \<Psi>\<^sub>2 \<nabla> n\<^sub>2 \<rbrakk>\<rbrakk>\<^sub>T\<^sub>E\<^sub>S\<^sub>L \<inter> \<lbrakk>\<lbrakk> \<Phi>\<^sub>2 \<nabla> Suc n\<^sub>2 \<rbrakk>\<rbrakk>\<^sub>T\<^sub>E\<^sub>S\<^sub>L \<subseteq> \<lbrakk>\<lbrakk> \<Gamma>\<^sub>1 \<rbrakk>\<rbrakk>\<^sub>s\<^sub>y\<^sub>m\<^sub>r\<^sub>u\<^sub>n \<inter> \<lbrakk>\<lbrakk> \<Psi>\<^sub>1 \<nabla> n\<^sub>1 \<rbrakk>\<rbrakk>\<^sub>T\<^sub>E\<^sub>S\<^sub>L \<inter> \<lbrakk>\<lbrakk> \<Phi>\<^sub>1 \<nabla> Suc n\<^sub>1 \<rbrakk>\<rbrakk>\<^sub>T\<^sub>E\<^sub>S\<^sub>L"
-    proof -
-    fix K\<^sub>1 :: clock and n :: nat and \<Gamma> :: "constr list" and \<delta>\<tau> :: tag_const and K\<^sub>2 :: clock and K\<^sub>3 :: clock and \<Psi> :: TESL_formula and \<Phi> :: TESL_formula
-    assume a1: "(\<Gamma>\<^sub>1, n\<^sub>1 \<turnstile> \<Psi>\<^sub>1 \<triangleright> \<Phi>\<^sub>1) = (\<Gamma>, n \<turnstile> (K\<^sub>1 time-delayed by \<delta>\<tau> on K\<^sub>2 implies K\<^sub>3) # \<Psi> \<triangleright> \<Phi>)"
-    assume a2: "(\<Gamma>\<^sub>2, n\<^sub>2 \<turnstile> \<Psi>\<^sub>2 \<triangleright> \<Phi>\<^sub>2) = (K\<^sub>1 \<Up> n # \<Gamma>, n \<turnstile> (K\<^sub>3 sporadic \<lfloor> \<tau>\<^sub>v\<^sub>a\<^sub>r (K\<^sub>2, n) \<oplus> \<delta>\<tau> \<rfloor> on K\<^sub>2) # \<Psi> \<triangleright> (K\<^sub>1 time-delayed by \<delta>\<tau> on K\<^sub>2 implies K\<^sub>3) # \<Phi>)"
-    have tdby_cases_corrollary: "\<lbrakk> K\<^sub>1 time-delayed by \<delta>\<tau> on K\<^sub>2 implies K\<^sub>3 \<nabla> n \<rbrakk>\<^sub>T\<^sub>E\<^sub>S\<^sub>L \<supseteq>
-        \<lbrakk> K\<^sub>1 \<Up> n \<rbrakk>\<^sub>s\<^sub>y\<^sub>m\<^sub>r\<^sub>u\<^sub>n \<inter> \<lbrakk> K\<^sub>3 sporadic \<lfloor>\<tau>\<^sub>v\<^sub>a\<^sub>r(K\<^sub>2, n) \<oplus> \<delta>\<tau>\<rfloor> on K\<^sub>2 \<nabla> n \<rbrakk>\<^sub>T\<^sub>E\<^sub>S\<^sub>L \<inter> \<lbrakk> K\<^sub>1 time-delayed by \<delta>\<tau> on K\<^sub>2 implies K\<^sub>3 \<nabla> Suc n \<rbrakk>\<^sub>T\<^sub>E\<^sub>S\<^sub>L"
-      using TESL_interp_at_index_timedelayed_cases by blast
-    then show "\<lbrakk>\<lbrakk> \<Gamma>\<^sub>2 \<rbrakk>\<rbrakk>\<^sub>s\<^sub>y\<^sub>m\<^sub>r\<^sub>u\<^sub>n \<inter> \<lbrakk>\<lbrakk> \<Psi>\<^sub>2 \<nabla> n\<^sub>2 \<rbrakk>\<rbrakk>\<^sub>T\<^sub>E\<^sub>S\<^sub>L \<inter> \<lbrakk>\<lbrakk> \<Phi>\<^sub>2 \<nabla> Suc n\<^sub>2 \<rbrakk>\<rbrakk>\<^sub>T\<^sub>E\<^sub>S\<^sub>L \<subseteq> \<lbrakk>\<lbrakk> \<Gamma>\<^sub>1 \<rbrakk>\<rbrakk>\<^sub>s\<^sub>y\<^sub>m\<^sub>r\<^sub>u\<^sub>n \<inter> \<lbrakk>\<lbrakk> \<Psi>\<^sub>1 \<nabla> n\<^sub>1 \<rbrakk>\<rbrakk>\<^sub>T\<^sub>E\<^sub>S\<^sub>L \<inter> \<lbrakk>\<lbrakk> \<Phi>\<^sub>1 \<nabla> Suc n\<^sub>1 \<rbrakk>\<rbrakk>\<^sub>T\<^sub>E\<^sub>S\<^sub>L"
-      using a1 a2 by auto
+  show "\<And>\<Gamma>\<^sub>1' n\<^sub>1' \<Psi>\<^sub>1' \<Phi>\<^sub>1' \<Gamma>\<^sub>2' n\<^sub>2' \<Psi>\<^sub>2' \<Phi>\<^sub>2'.
+       \<Gamma>\<^sub>1, n\<^sub>1 \<turnstile> \<Psi>\<^sub>1 \<triangleright> \<Phi>\<^sub>1 = \<Gamma>\<^sub>1', n\<^sub>1' \<turnstile> \<Psi>\<^sub>1' \<triangleright> \<Phi>\<^sub>1' \<Longrightarrow>
+       \<Gamma>\<^sub>2, n\<^sub>2 \<turnstile> \<Psi>\<^sub>2 \<triangleright> \<Phi>\<^sub>2 = \<Gamma>\<^sub>2', n\<^sub>2' \<turnstile> \<Psi>\<^sub>2' \<triangleright> \<Phi>\<^sub>2' \<Longrightarrow>
+       \<Gamma>\<^sub>1', n\<^sub>1' \<turnstile> \<Psi>\<^sub>1' \<triangleright> \<Phi>\<^sub>1' \<hookrightarrow>\<^sub>i \<Gamma>\<^sub>2', n\<^sub>2' \<turnstile> \<Psi>\<^sub>2' \<triangleright> \<Phi>\<^sub>2' \<Longrightarrow>
+       \<lbrakk>\<lbrakk> \<Gamma>\<^sub>2 \<rbrakk>\<rbrakk>\<^sub>s\<^sub>y\<^sub>m\<^sub>r\<^sub>u\<^sub>n \<inter> \<lbrakk>\<lbrakk> \<Psi>\<^sub>2 \<rbrakk>\<rbrakk>\<^sub>T\<^sub>E\<^sub>S\<^sub>L\<^bsup>\<ge> n\<^sub>2\<^esup> \<inter> \<lbrakk>\<lbrakk> \<Phi>\<^sub>2 \<rbrakk>\<rbrakk>\<^sub>T\<^sub>E\<^sub>S\<^sub>L\<^bsup>\<ge> Suc n\<^sub>2\<^esup>
+       \<subseteq> \<lbrakk>\<lbrakk> \<Gamma>\<^sub>1 \<rbrakk>\<rbrakk>\<^sub>s\<^sub>y\<^sub>m\<^sub>r\<^sub>u\<^sub>n \<inter> \<lbrakk>\<lbrakk> \<Psi>\<^sub>1 \<rbrakk>\<rbrakk>\<^sub>T\<^sub>E\<^sub>S\<^sub>L\<^bsup>\<ge> n\<^sub>1\<^esup> \<inter> \<lbrakk>\<lbrakk> \<Phi>\<^sub>1 \<rbrakk>\<rbrakk>\<^sub>T\<^sub>E\<^sub>S\<^sub>L\<^bsup>\<ge> Suc n\<^sub>1\<^esup>"
+    by (erule operational_semantics_intro.cases, auto)
+  show "\<And>\<Gamma>\<^sub>1' n\<^sub>1' \<Psi>\<^sub>1' \<Phi>\<^sub>1' \<Gamma>\<^sub>2' n\<^sub>2' \<Psi>\<^sub>2' \<Phi>\<^sub>2'.
+       \<Gamma>\<^sub>1, n\<^sub>1 \<turnstile> \<Psi>\<^sub>1 \<triangleright> \<Phi>\<^sub>1 = \<Gamma>\<^sub>1', n\<^sub>1' \<turnstile> \<Psi>\<^sub>1' \<triangleright> \<Phi>\<^sub>1' \<Longrightarrow>
+       \<Gamma>\<^sub>2, n\<^sub>2 \<turnstile> \<Psi>\<^sub>2 \<triangleright> \<Phi>\<^sub>2 = \<Gamma>\<^sub>2', n\<^sub>2' \<turnstile> \<Psi>\<^sub>2' \<triangleright> \<Phi>\<^sub>2' \<Longrightarrow>
+       \<Gamma>\<^sub>1', n\<^sub>1' \<turnstile> \<Psi>\<^sub>1' \<triangleright> \<Phi>\<^sub>1' \<hookrightarrow>\<^sub>e \<Gamma>\<^sub>2', n\<^sub>2' \<turnstile> \<Psi>\<^sub>2' \<triangleright> \<Phi>\<^sub>2' \<Longrightarrow>
+       \<lbrakk>\<lbrakk> \<Gamma>\<^sub>2 \<rbrakk>\<rbrakk>\<^sub>s\<^sub>y\<^sub>m\<^sub>r\<^sub>u\<^sub>n \<inter> \<lbrakk>\<lbrakk> \<Psi>\<^sub>2 \<rbrakk>\<rbrakk>\<^sub>T\<^sub>E\<^sub>S\<^sub>L\<^bsup>\<ge> n\<^sub>2\<^esup> \<inter> \<lbrakk>\<lbrakk> \<Phi>\<^sub>2 \<rbrakk>\<rbrakk>\<^sub>T\<^sub>E\<^sub>S\<^sub>L\<^bsup>\<ge> Suc n\<^sub>2\<^esup>
+       \<subseteq> \<lbrakk>\<lbrakk> \<Gamma>\<^sub>1 \<rbrakk>\<rbrakk>\<^sub>s\<^sub>y\<^sub>m\<^sub>r\<^sub>u\<^sub>n \<inter> \<lbrakk>\<lbrakk> \<Psi>\<^sub>1 \<rbrakk>\<rbrakk>\<^sub>T\<^sub>E\<^sub>S\<^sub>L\<^bsup>\<ge> n\<^sub>1\<^esup> \<inter> \<lbrakk>\<lbrakk> \<Phi>\<^sub>1 \<rbrakk>\<rbrakk>\<^sub>T\<^sub>E\<^sub>S\<^sub>L\<^bsup>\<ge> Suc n\<^sub>1\<^esup>"
+    proof (erule operational_semantics_elim.cases)
+    show "\<And>\<Gamma>\<^sub>1' n\<^sub>1' \<Psi>\<^sub>1' \<Phi>\<^sub>1' \<Gamma>\<^sub>2' n\<^sub>2' \<Psi>\<^sub>2' \<Phi>\<^sub>2' \<Gamma> n K \<tau> \<Psi> \<Phi>.
+       (\<Gamma>\<^sub>1, n\<^sub>1 \<turnstile> \<Psi>\<^sub>1 \<triangleright> \<Phi>\<^sub>1) = (\<Gamma>\<^sub>1', n\<^sub>1' \<turnstile> \<Psi>\<^sub>1' \<triangleright> \<Phi>\<^sub>1') \<Longrightarrow>
+       (\<Gamma>\<^sub>2, n\<^sub>2 \<turnstile> \<Psi>\<^sub>2 \<triangleright> \<Phi>\<^sub>2) = (\<Gamma>\<^sub>2', n\<^sub>2' \<turnstile> \<Psi>\<^sub>2' \<triangleright> \<Phi>\<^sub>2') \<Longrightarrow>
+       (\<Gamma>\<^sub>1', n\<^sub>1' \<turnstile> \<Psi>\<^sub>1' \<triangleright> \<Phi>\<^sub>1') = (\<Gamma>, n \<turnstile> (K sporadic \<tau>) # \<Psi> \<triangleright> \<Phi>) \<Longrightarrow>
+       (\<Gamma>\<^sub>2', n\<^sub>2' \<turnstile> \<Psi>\<^sub>2' \<triangleright> \<Phi>\<^sub>2') = (\<Gamma>, n \<turnstile> \<Psi> \<triangleright> (K sporadic \<tau>) # \<Phi>) \<Longrightarrow>
+       \<lbrakk>\<lbrakk> \<Gamma>\<^sub>2 \<rbrakk>\<rbrakk>\<^sub>s\<^sub>y\<^sub>m\<^sub>r\<^sub>u\<^sub>n \<inter> \<lbrakk>\<lbrakk> \<Psi>\<^sub>2 \<rbrakk>\<rbrakk>\<^sub>T\<^sub>E\<^sub>S\<^sub>L\<^bsup>\<ge> n\<^sub>2\<^esup> \<inter> \<lbrakk>\<lbrakk> \<Phi>\<^sub>2 \<rbrakk>\<rbrakk>\<^sub>T\<^sub>E\<^sub>S\<^sub>L\<^bsup>\<ge> Suc n\<^sub>2\<^esup>
+       \<subseteq> \<lbrakk>\<lbrakk> \<Gamma>\<^sub>1 \<rbrakk>\<rbrakk>\<^sub>s\<^sub>y\<^sub>m\<^sub>r\<^sub>u\<^sub>n \<inter> \<lbrakk>\<lbrakk> \<Psi>\<^sub>1 \<rbrakk>\<rbrakk>\<^sub>T\<^sub>E\<^sub>S\<^sub>L\<^bsup>\<ge> n\<^sub>1\<^esup> \<inter> \<lbrakk>\<lbrakk> \<Phi>\<^sub>1 \<rbrakk>\<rbrakk>\<^sub>T\<^sub>E\<^sub>S\<^sub>L\<^bsup>\<ge> Suc n\<^sub>1\<^esup>"
+      using HeronConf_interp_at_index_sporadic_cases by auto
+    show "\<And>\<Gamma>\<^sub>1' n\<^sub>1' \<Psi>\<^sub>1' \<Phi>\<^sub>1' \<Gamma>\<^sub>2' n\<^sub>2' \<Psi>\<^sub>2' \<Phi>\<^sub>2' \<Gamma> n K \<tau> \<Psi> \<Phi>.
+       (\<Gamma>\<^sub>1, n\<^sub>1 \<turnstile> \<Psi>\<^sub>1 \<triangleright> \<Phi>\<^sub>1) = (\<Gamma>\<^sub>1', n\<^sub>1' \<turnstile> \<Psi>\<^sub>1' \<triangleright> \<Phi>\<^sub>1') \<Longrightarrow>
+       (\<Gamma>\<^sub>2, n\<^sub>2 \<turnstile> \<Psi>\<^sub>2 \<triangleright> \<Phi>\<^sub>2) = (\<Gamma>\<^sub>2', n\<^sub>2' \<turnstile> \<Psi>\<^sub>2' \<triangleright> \<Phi>\<^sub>2') \<Longrightarrow>
+       (\<Gamma>\<^sub>1', n\<^sub>1' \<turnstile> \<Psi>\<^sub>1' \<triangleright> \<Phi>\<^sub>1') = (\<Gamma>, n \<turnstile> (K sporadic \<tau>) # \<Psi> \<triangleright> \<Phi>) \<Longrightarrow>
+       (\<Gamma>\<^sub>2', n\<^sub>2' \<turnstile> \<Psi>\<^sub>2' \<triangleright> \<Phi>\<^sub>2') = (K \<Up> n # K \<Down> n @ \<lfloor> \<tau> \<rfloor> # \<Gamma>, n \<turnstile> \<Psi> \<triangleright> \<Phi>) \<Longrightarrow>
+       \<lbrakk>\<lbrakk> \<Gamma>\<^sub>2 \<rbrakk>\<rbrakk>\<^sub>s\<^sub>y\<^sub>m\<^sub>r\<^sub>u\<^sub>n \<inter> \<lbrakk>\<lbrakk> \<Psi>\<^sub>2 \<rbrakk>\<rbrakk>\<^sub>T\<^sub>E\<^sub>S\<^sub>L\<^bsup>\<ge> n\<^sub>2\<^esup> \<inter> \<lbrakk>\<lbrakk> \<Phi>\<^sub>2 \<rbrakk>\<rbrakk>\<^sub>T\<^sub>E\<^sub>S\<^sub>L\<^bsup>\<ge> Suc n\<^sub>2\<^esup>
+       \<subseteq> \<lbrakk>\<lbrakk> \<Gamma>\<^sub>1 \<rbrakk>\<rbrakk>\<^sub>s\<^sub>y\<^sub>m\<^sub>r\<^sub>u\<^sub>n \<inter> \<lbrakk>\<lbrakk> \<Psi>\<^sub>1 \<rbrakk>\<rbrakk>\<^sub>T\<^sub>E\<^sub>S\<^sub>L\<^bsup>\<ge> n\<^sub>1\<^esup> \<inter> \<lbrakk>\<lbrakk> \<Phi>\<^sub>1 \<rbrakk>\<rbrakk>\<^sub>T\<^sub>E\<^sub>S\<^sub>L\<^bsup>\<ge> Suc n\<^sub>1\<^esup>"
+      using HeronConf_interp_at_index_sporadic_cases by auto
+    show "\<And>\<Gamma>\<^sub>1' n\<^sub>1' \<Psi>\<^sub>1' \<Phi>\<^sub>1' \<Gamma>\<^sub>2' n\<^sub>2' \<Psi>\<^sub>2' \<Phi>\<^sub>2' \<Gamma> n K\<^sub>1 \<tau> K\<^sub>2 \<Psi> \<Phi>.
+       (\<Gamma>\<^sub>1, n\<^sub>1 \<turnstile> \<Psi>\<^sub>1 \<triangleright> \<Phi>\<^sub>1) = (\<Gamma>\<^sub>1', n\<^sub>1' \<turnstile> \<Psi>\<^sub>1' \<triangleright> \<Phi>\<^sub>1') \<Longrightarrow>
+       (\<Gamma>\<^sub>2, n\<^sub>2 \<turnstile> \<Psi>\<^sub>2 \<triangleright> \<Phi>\<^sub>2) = (\<Gamma>\<^sub>2', n\<^sub>2' \<turnstile> \<Psi>\<^sub>2' \<triangleright> \<Phi>\<^sub>2') \<Longrightarrow>
+       (\<Gamma>\<^sub>1', n\<^sub>1' \<turnstile> \<Psi>\<^sub>1' \<triangleright> \<Phi>\<^sub>1') = (\<Gamma>, n \<turnstile> (K\<^sub>1 sporadic \<tau> on K\<^sub>2) # \<Psi> \<triangleright> \<Phi>) \<Longrightarrow>
+       (\<Gamma>\<^sub>2', n\<^sub>2' \<turnstile> \<Psi>\<^sub>2' \<triangleright> \<Phi>\<^sub>2') = (\<Gamma>, n \<turnstile> \<Psi> \<triangleright> (K\<^sub>1 sporadic \<tau> on K\<^sub>2) # \<Phi>) \<Longrightarrow>
+       \<lbrakk>\<lbrakk> \<Gamma>\<^sub>2 \<rbrakk>\<rbrakk>\<^sub>s\<^sub>y\<^sub>m\<^sub>r\<^sub>u\<^sub>n \<inter> \<lbrakk>\<lbrakk> \<Psi>\<^sub>2 \<rbrakk>\<rbrakk>\<^sub>T\<^sub>E\<^sub>S\<^sub>L\<^bsup>\<ge> n\<^sub>2\<^esup> \<inter> \<lbrakk>\<lbrakk> \<Phi>\<^sub>2 \<rbrakk>\<rbrakk>\<^sub>T\<^sub>E\<^sub>S\<^sub>L\<^bsup>\<ge> Suc n\<^sub>2\<^esup>
+       \<subseteq> \<lbrakk>\<lbrakk> \<Gamma>\<^sub>1 \<rbrakk>\<rbrakk>\<^sub>s\<^sub>y\<^sub>m\<^sub>r\<^sub>u\<^sub>n \<inter> \<lbrakk>\<lbrakk> \<Psi>\<^sub>1 \<rbrakk>\<rbrakk>\<^sub>T\<^sub>E\<^sub>S\<^sub>L\<^bsup>\<ge> n\<^sub>1\<^esup> \<inter> \<lbrakk>\<lbrakk> \<Phi>\<^sub>1 \<rbrakk>\<rbrakk>\<^sub>T\<^sub>E\<^sub>S\<^sub>L\<^bsup>\<ge> Suc n\<^sub>1\<^esup>"
+      using HeronConf_interp_at_index_sporadicon_cases by auto
+    show "\<And>\<Gamma>\<^sub>1' n\<^sub>1' \<Psi>\<^sub>1' \<Phi>\<^sub>1' \<Gamma>\<^sub>2' n\<^sub>2' \<Psi>\<^sub>2' \<Phi>\<^sub>2' \<Gamma> n K\<^sub>1 \<tau> K\<^sub>2 \<Psi> \<Phi>.
+       (\<Gamma>\<^sub>1, n\<^sub>1 \<turnstile> \<Psi>\<^sub>1 \<triangleright> \<Phi>\<^sub>1) = (\<Gamma>\<^sub>1', n\<^sub>1' \<turnstile> \<Psi>\<^sub>1' \<triangleright> \<Phi>\<^sub>1') \<Longrightarrow>
+       (\<Gamma>\<^sub>2, n\<^sub>2 \<turnstile> \<Psi>\<^sub>2 \<triangleright> \<Phi>\<^sub>2) = (\<Gamma>\<^sub>2', n\<^sub>2' \<turnstile> \<Psi>\<^sub>2' \<triangleright> \<Phi>\<^sub>2') \<Longrightarrow>
+       (\<Gamma>\<^sub>1', n\<^sub>1' \<turnstile> \<Psi>\<^sub>1' \<triangleright> \<Phi>\<^sub>1') = (\<Gamma>, n \<turnstile> (K\<^sub>1 sporadic \<tau> on K\<^sub>2) # \<Psi> \<triangleright> \<Phi>) \<Longrightarrow>
+       (\<Gamma>\<^sub>2', n\<^sub>2' \<turnstile> \<Psi>\<^sub>2' \<triangleright> \<Phi>\<^sub>2') = (K\<^sub>1 \<Up> n # K\<^sub>2 \<Down> n @ \<tau> # \<Gamma>, n \<turnstile> \<Psi> \<triangleright> \<Phi>) \<Longrightarrow>
+       \<lbrakk>\<lbrakk> \<Gamma>\<^sub>2 \<rbrakk>\<rbrakk>\<^sub>s\<^sub>y\<^sub>m\<^sub>r\<^sub>u\<^sub>n \<inter> \<lbrakk>\<lbrakk> \<Psi>\<^sub>2 \<rbrakk>\<rbrakk>\<^sub>T\<^sub>E\<^sub>S\<^sub>L\<^bsup>\<ge> n\<^sub>2\<^esup> \<inter> \<lbrakk>\<lbrakk> \<Phi>\<^sub>2 \<rbrakk>\<rbrakk>\<^sub>T\<^sub>E\<^sub>S\<^sub>L\<^bsup>\<ge> Suc n\<^sub>2\<^esup>
+       \<subseteq> \<lbrakk>\<lbrakk> \<Gamma>\<^sub>1 \<rbrakk>\<rbrakk>\<^sub>s\<^sub>y\<^sub>m\<^sub>r\<^sub>u\<^sub>n \<inter> \<lbrakk>\<lbrakk> \<Psi>\<^sub>1 \<rbrakk>\<rbrakk>\<^sub>T\<^sub>E\<^sub>S\<^sub>L\<^bsup>\<ge> n\<^sub>1\<^esup> \<inter> \<lbrakk>\<lbrakk> \<Phi>\<^sub>1 \<rbrakk>\<rbrakk>\<^sub>T\<^sub>E\<^sub>S\<^sub>L\<^bsup>\<ge> Suc n\<^sub>1\<^esup>"
+      using HeronConf_interp_at_index_sporadicon_cases by auto
+    show "\<And>\<Gamma>\<^sub>1' n\<^sub>1' \<Psi>\<^sub>1' \<Phi>\<^sub>1' \<Gamma>\<^sub>2' n\<^sub>2' \<Psi>\<^sub>2' \<Phi>\<^sub>2' \<Gamma> n K\<^sub>1 \<alpha> K\<^sub>2 \<beta> \<Psi> \<Phi>.
+       (\<Gamma>\<^sub>1, n\<^sub>1 \<turnstile> \<Psi>\<^sub>1 \<triangleright> \<Phi>\<^sub>1) = \<Gamma>\<^sub>1', n\<^sub>1' \<turnstile> \<Psi>\<^sub>1' \<triangleright> \<Phi>\<^sub>1' \<Longrightarrow>
+       (\<Gamma>\<^sub>2, n\<^sub>2 \<turnstile> \<Psi>\<^sub>2 \<triangleright> \<Phi>\<^sub>2) = \<Gamma>\<^sub>2', n\<^sub>2' \<turnstile> \<Psi>\<^sub>2' \<triangleright> \<Phi>\<^sub>2' \<Longrightarrow>
+       (\<Gamma>\<^sub>1', n\<^sub>1' \<turnstile> \<Psi>\<^sub>1' \<triangleright> \<Phi>\<^sub>1') = \<Gamma>, n \<turnstile> (tag-relation K\<^sub>1 = \<alpha> * K\<^sub>2 + \<beta>) # \<Psi> \<triangleright> \<Phi> \<Longrightarrow>
+       (\<Gamma>\<^sub>2', n\<^sub>2' \<turnstile> \<Psi>\<^sub>2' \<triangleright> \<Phi>\<^sub>2') =
+       \<tau>\<^sub>v\<^sub>a\<^sub>r (K\<^sub>1, n) \<doteq> \<alpha> * \<tau>\<^sub>v\<^sub>a\<^sub>r (K\<^sub>2, n) + \<beta> #
+       \<Gamma>, n \<turnstile> \<Psi> \<triangleright> (tag-relation K\<^sub>1 = \<alpha> * K\<^sub>2 + \<beta>) # \<Phi> \<Longrightarrow>
+       \<lbrakk>\<lbrakk> \<Gamma>\<^sub>2 \<rbrakk>\<rbrakk>\<^sub>s\<^sub>y\<^sub>m\<^sub>r\<^sub>u\<^sub>n \<inter> \<lbrakk>\<lbrakk> \<Psi>\<^sub>2 \<rbrakk>\<rbrakk>\<^sub>T\<^sub>E\<^sub>S\<^sub>L\<^bsup>\<ge> n\<^sub>2\<^esup> \<inter> \<lbrakk>\<lbrakk> \<Phi>\<^sub>2 \<rbrakk>\<rbrakk>\<^sub>T\<^sub>E\<^sub>S\<^sub>L\<^bsup>\<ge> Suc n\<^sub>2\<^esup>
+       \<subseteq> \<lbrakk>\<lbrakk> \<Gamma>\<^sub>1 \<rbrakk>\<rbrakk>\<^sub>s\<^sub>y\<^sub>m\<^sub>r\<^sub>u\<^sub>n \<inter> \<lbrakk>\<lbrakk> \<Psi>\<^sub>1 \<rbrakk>\<rbrakk>\<^sub>T\<^sub>E\<^sub>S\<^sub>L\<^bsup>\<ge> n\<^sub>1\<^esup> \<inter> \<lbrakk>\<lbrakk> \<Phi>\<^sub>1 \<rbrakk>\<rbrakk>\<^sub>T\<^sub>E\<^sub>S\<^sub>L\<^bsup>\<ge> Suc n\<^sub>1\<^esup>"
+      using HeronConf_interp_at_index_tagrel_cases by auto
+    show "\<And>\<Gamma>\<^sub>1' n\<^sub>1' \<Psi>\<^sub>1' \<Phi>\<^sub>1' \<Gamma>\<^sub>2' n\<^sub>2' \<Psi>\<^sub>2' \<Phi>\<^sub>2' \<Gamma> n K\<^sub>1 K\<^sub>2 \<Psi> \<Phi>.
+       (\<Gamma>\<^sub>1, n\<^sub>1 \<turnstile> \<Psi>\<^sub>1 \<triangleright> \<Phi>\<^sub>1) = \<Gamma>\<^sub>1', n\<^sub>1' \<turnstile> \<Psi>\<^sub>1' \<triangleright> \<Phi>\<^sub>1' \<Longrightarrow>
+       (\<Gamma>\<^sub>2, n\<^sub>2 \<turnstile> \<Psi>\<^sub>2 \<triangleright> \<Phi>\<^sub>2) = \<Gamma>\<^sub>2', n\<^sub>2' \<turnstile> \<Psi>\<^sub>2' \<triangleright> \<Phi>\<^sub>2' \<Longrightarrow>
+       (\<Gamma>\<^sub>1', n\<^sub>1' \<turnstile> \<Psi>\<^sub>1' \<triangleright> \<Phi>\<^sub>1') = \<Gamma>, n \<turnstile> (K\<^sub>1 implies K\<^sub>2) # \<Psi> \<triangleright> \<Phi> \<Longrightarrow>
+       (\<Gamma>\<^sub>2', n\<^sub>2' \<turnstile> \<Psi>\<^sub>2' \<triangleright> \<Phi>\<^sub>2') = K\<^sub>1 \<not>\<Up> n # \<Gamma>, n \<turnstile> \<Psi> \<triangleright> (K\<^sub>1 implies K\<^sub>2) # \<Phi> \<Longrightarrow>
+       \<lbrakk>\<lbrakk> \<Gamma>\<^sub>2 \<rbrakk>\<rbrakk>\<^sub>s\<^sub>y\<^sub>m\<^sub>r\<^sub>u\<^sub>n \<inter> \<lbrakk>\<lbrakk> \<Psi>\<^sub>2 \<rbrakk>\<rbrakk>\<^sub>T\<^sub>E\<^sub>S\<^sub>L\<^bsup>\<ge> n\<^sub>2\<^esup> \<inter> \<lbrakk>\<lbrakk> \<Phi>\<^sub>2 \<rbrakk>\<rbrakk>\<^sub>T\<^sub>E\<^sub>S\<^sub>L\<^bsup>\<ge> Suc n\<^sub>2\<^esup>
+       \<subseteq> \<lbrakk>\<lbrakk> \<Gamma>\<^sub>1 \<rbrakk>\<rbrakk>\<^sub>s\<^sub>y\<^sub>m\<^sub>r\<^sub>u\<^sub>n \<inter> \<lbrakk>\<lbrakk> \<Psi>\<^sub>1 \<rbrakk>\<rbrakk>\<^sub>T\<^sub>E\<^sub>S\<^sub>L\<^bsup>\<ge> n\<^sub>1\<^esup> \<inter> \<lbrakk>\<lbrakk> \<Phi>\<^sub>1 \<rbrakk>\<rbrakk>\<^sub>T\<^sub>E\<^sub>S\<^sub>L\<^bsup>\<ge> Suc n\<^sub>1\<^esup>"
+      using HeronConf_interp_at_index_implies_cases by auto
+    show "\<And>\<Gamma>\<^sub>1' n\<^sub>1' \<Psi>\<^sub>1' \<Phi>\<^sub>1' \<Gamma>\<^sub>2' n\<^sub>2' \<Psi>\<^sub>2' \<Phi>\<^sub>2' \<Gamma> n K\<^sub>1 K\<^sub>2 \<Psi> \<Phi>.
+       (\<Gamma>\<^sub>1, n\<^sub>1 \<turnstile> \<Psi>\<^sub>1 \<triangleright> \<Phi>\<^sub>1) = (\<Gamma>\<^sub>1', n\<^sub>1' \<turnstile> \<Psi>\<^sub>1' \<triangleright> \<Phi>\<^sub>1') \<Longrightarrow>
+       (\<Gamma>\<^sub>2, n\<^sub>2 \<turnstile> \<Psi>\<^sub>2 \<triangleright> \<Phi>\<^sub>2) = (\<Gamma>\<^sub>2', n\<^sub>2' \<turnstile> \<Psi>\<^sub>2' \<triangleright> \<Phi>\<^sub>2') \<Longrightarrow>
+       (\<Gamma>\<^sub>1', n\<^sub>1' \<turnstile> \<Psi>\<^sub>1' \<triangleright> \<Phi>\<^sub>1') = (\<Gamma>, n \<turnstile> (K\<^sub>1 implies K\<^sub>2) # \<Psi> \<triangleright> \<Phi>) \<Longrightarrow>
+       (\<Gamma>\<^sub>2', n\<^sub>2' \<turnstile> \<Psi>\<^sub>2' \<triangleright> \<Phi>\<^sub>2') = (K\<^sub>1 \<Up> n # K\<^sub>2 \<Up> n # \<Gamma>, n \<turnstile> \<Psi> \<triangleright> (K\<^sub>1 implies K\<^sub>2) # \<Phi>) \<Longrightarrow>
+       \<lbrakk>\<lbrakk> \<Gamma>\<^sub>2 \<rbrakk>\<rbrakk>\<^sub>s\<^sub>y\<^sub>m\<^sub>r\<^sub>u\<^sub>n \<inter> \<lbrakk>\<lbrakk> \<Psi>\<^sub>2 \<rbrakk>\<rbrakk>\<^sub>T\<^sub>E\<^sub>S\<^sub>L\<^bsup>\<ge> n\<^sub>2\<^esup> \<inter> \<lbrakk>\<lbrakk> \<Phi>\<^sub>2 \<rbrakk>\<rbrakk>\<^sub>T\<^sub>E\<^sub>S\<^sub>L\<^bsup>\<ge> Suc n\<^sub>2\<^esup>
+       \<subseteq> \<lbrakk>\<lbrakk> \<Gamma>\<^sub>1 \<rbrakk>\<rbrakk>\<^sub>s\<^sub>y\<^sub>m\<^sub>r\<^sub>u\<^sub>n \<inter> \<lbrakk>\<lbrakk> \<Psi>\<^sub>1 \<rbrakk>\<rbrakk>\<^sub>T\<^sub>E\<^sub>S\<^sub>L\<^bsup>\<ge> n\<^sub>1\<^esup> \<inter> \<lbrakk>\<lbrakk> \<Phi>\<^sub>1 \<rbrakk>\<rbrakk>\<^sub>T\<^sub>E\<^sub>S\<^sub>L\<^bsup>\<ge> Suc n\<^sub>1\<^esup>"
+      using HeronConf_interp_at_index_implies_cases by auto
+    show "\<And>\<Gamma>\<^sub>1' n\<^sub>1' \<Psi>\<^sub>1' \<Phi>\<^sub>1' \<Gamma>\<^sub>2' n\<^sub>2' \<Psi>\<^sub>2' \<Phi>\<^sub>2' \<Gamma> n K\<^sub>1 \<delta>\<tau> K\<^sub>2 K\<^sub>3 \<Psi> \<Phi>.
+       (\<Gamma>\<^sub>1, n\<^sub>1 \<turnstile> \<Psi>\<^sub>1 \<triangleright> \<Phi>\<^sub>1) = (\<Gamma>\<^sub>1', n\<^sub>1' \<turnstile> \<Psi>\<^sub>1' \<triangleright> \<Phi>\<^sub>1') \<Longrightarrow>
+       (\<Gamma>\<^sub>2, n\<^sub>2 \<turnstile> \<Psi>\<^sub>2 \<triangleright> \<Phi>\<^sub>2) = (\<Gamma>\<^sub>2', n\<^sub>2' \<turnstile> \<Psi>\<^sub>2' \<triangleright> \<Phi>\<^sub>2') \<Longrightarrow>
+       (\<Gamma>\<^sub>1', n\<^sub>1' \<turnstile> \<Psi>\<^sub>1' \<triangleright> \<Phi>\<^sub>1') = \<Gamma>, n \<turnstile> (K\<^sub>1 time-delayed by \<delta>\<tau> on K\<^sub>2 implies K\<^sub>3) # \<Psi> \<triangleright> \<Phi> \<Longrightarrow>
+       (\<Gamma>\<^sub>2', n\<^sub>2' \<turnstile> \<Psi>\<^sub>2' \<triangleright> \<Phi>\<^sub>2') =
+       K\<^sub>1 \<not>\<Up> n # \<Gamma>, n \<turnstile> \<Psi> \<triangleright> (K\<^sub>1 time-delayed by \<delta>\<tau> on K\<^sub>2 implies K\<^sub>3) # \<Phi> \<Longrightarrow>
+       \<lbrakk>\<lbrakk> \<Gamma>\<^sub>2 \<rbrakk>\<rbrakk>\<^sub>s\<^sub>y\<^sub>m\<^sub>r\<^sub>u\<^sub>n \<inter> \<lbrakk>\<lbrakk> \<Psi>\<^sub>2 \<rbrakk>\<rbrakk>\<^sub>T\<^sub>E\<^sub>S\<^sub>L\<^bsup>\<ge> n\<^sub>2\<^esup> \<inter> \<lbrakk>\<lbrakk> \<Phi>\<^sub>2 \<rbrakk>\<rbrakk>\<^sub>T\<^sub>E\<^sub>S\<^sub>L\<^bsup>\<ge> Suc n\<^sub>2\<^esup>
+       \<subseteq> \<lbrakk>\<lbrakk> \<Gamma>\<^sub>1 \<rbrakk>\<rbrakk>\<^sub>s\<^sub>y\<^sub>m\<^sub>r\<^sub>u\<^sub>n \<inter> \<lbrakk>\<lbrakk> \<Psi>\<^sub>1 \<rbrakk>\<rbrakk>\<^sub>T\<^sub>E\<^sub>S\<^sub>L\<^bsup>\<ge> n\<^sub>1\<^esup> \<inter> \<lbrakk>\<lbrakk> \<Phi>\<^sub>1 \<rbrakk>\<rbrakk>\<^sub>T\<^sub>E\<^sub>S\<^sub>L\<^bsup>\<ge> Suc n\<^sub>1\<^esup>"
+      using HeronConf_interp_at_index_timedelayed_cases by auto
+    show "\<And>\<Gamma>\<^sub>1' n\<^sub>1' \<Psi>\<^sub>1' \<Phi>\<^sub>1' \<Gamma>\<^sub>2' n\<^sub>2' \<Psi>\<^sub>2' \<Phi>\<^sub>2' \<Gamma> n K\<^sub>1 \<delta>\<tau> K\<^sub>2 K\<^sub>3 \<Psi> \<Phi>.
+       (\<Gamma>\<^sub>1, n\<^sub>1 \<turnstile> \<Psi>\<^sub>1 \<triangleright> \<Phi>\<^sub>1) = (\<Gamma>\<^sub>1', n\<^sub>1' \<turnstile> \<Psi>\<^sub>1' \<triangleright> \<Phi>\<^sub>1') \<Longrightarrow>
+       (\<Gamma>\<^sub>2, n\<^sub>2 \<turnstile> \<Psi>\<^sub>2 \<triangleright> \<Phi>\<^sub>2) = (\<Gamma>\<^sub>2', n\<^sub>2' \<turnstile> \<Psi>\<^sub>2' \<triangleright> \<Phi>\<^sub>2') \<Longrightarrow>
+       (\<Gamma>\<^sub>1', n\<^sub>1' \<turnstile> \<Psi>\<^sub>1' \<triangleright> \<Phi>\<^sub>1') = \<Gamma>, n \<turnstile> (K\<^sub>1 time-delayed by \<delta>\<tau> on K\<^sub>2 implies K\<^sub>3) # \<Psi> \<triangleright> \<Phi> \<Longrightarrow>
+       (\<Gamma>\<^sub>2', n\<^sub>2' \<turnstile> \<Psi>\<^sub>2' \<triangleright> \<Phi>\<^sub>2') =
+       K\<^sub>1 \<Up> n #
+       \<Gamma>, n \<turnstile> (K\<^sub>3 sporadic \<lfloor> \<tau>\<^sub>v\<^sub>a\<^sub>r (K\<^sub>2, n) \<oplus> \<delta>\<tau> \<rfloor> on K\<^sub>2) #
+               \<Psi> \<triangleright> (K\<^sub>1 time-delayed by \<delta>\<tau> on K\<^sub>2 implies K\<^sub>3) # \<Phi> \<Longrightarrow>
+       \<lbrakk>\<lbrakk> \<Gamma>\<^sub>2 \<rbrakk>\<rbrakk>\<^sub>s\<^sub>y\<^sub>m\<^sub>r\<^sub>u\<^sub>n \<inter> \<lbrakk>\<lbrakk> \<Psi>\<^sub>2 \<rbrakk>\<rbrakk>\<^sub>T\<^sub>E\<^sub>S\<^sub>L\<^bsup>\<ge> n\<^sub>2\<^esup> \<inter> \<lbrakk>\<lbrakk> \<Phi>\<^sub>2 \<rbrakk>\<rbrakk>\<^sub>T\<^sub>E\<^sub>S\<^sub>L\<^bsup>\<ge> Suc n\<^sub>2\<^esup>
+       \<subseteq> \<lbrakk>\<lbrakk> \<Gamma>\<^sub>1 \<rbrakk>\<rbrakk>\<^sub>s\<^sub>y\<^sub>m\<^sub>r\<^sub>u\<^sub>n \<inter> \<lbrakk>\<lbrakk> \<Psi>\<^sub>1 \<rbrakk>\<rbrakk>\<^sub>T\<^sub>E\<^sub>S\<^sub>L\<^bsup>\<ge> n\<^sub>1\<^esup> \<inter> \<lbrakk>\<lbrakk> \<Phi>\<^sub>1 \<rbrakk>\<rbrakk>\<^sub>T\<^sub>E\<^sub>S\<^sub>L\<^bsup>\<ge> Suc n\<^sub>1\<^esup>"
+      using HeronConf_interp_at_index_timedelayed_cases by auto
     qed
   qed
 
 theorem soundness':
   assumes "\<S>\<^sub>1 \<hookrightarrow> \<S>\<^sub>2"
-  shows "\<lbrakk> \<S>\<^sub>1 \<rbrakk>\<^sub>c\<^sub>o\<^sub>n\<^sub>f \<supseteq> \<lbrakk> \<S>\<^sub>2 \<rbrakk>\<^sub>c\<^sub>o\<^sub>n\<^sub>f"
+  shows "\<lbrakk> \<S>\<^sub>1 \<rbrakk>\<^sub>c\<^sub>o\<^sub>n\<^sub>f\<^sub>i\<^sub>g \<supseteq> \<lbrakk> \<S>\<^sub>2 \<rbrakk>\<^sub>c\<^sub>o\<^sub>n\<^sub>f\<^sub>i\<^sub>g"
   by (metis soundness HeronConf_interpretation.elims assms)
 
 theorem soundness_generalized:
   assumes "\<S>\<^sub>1 \<hookrightarrow>\<^bsup>n\<^esup> \<S>\<^sub>2"
-  shows "\<lbrakk> \<S>\<^sub>1 \<rbrakk>\<^sub>c\<^sub>o\<^sub>n\<^sub>f \<supseteq> \<lbrakk> \<S>\<^sub>2 \<rbrakk>\<^sub>c\<^sub>o\<^sub>n\<^sub>f"
+  shows "\<lbrakk> \<S>\<^sub>1 \<rbrakk>\<^sub>c\<^sub>o\<^sub>n\<^sub>f\<^sub>i\<^sub>g \<supseteq> \<lbrakk> \<S>\<^sub>2 \<rbrakk>\<^sub>c\<^sub>o\<^sub>n\<^sub>f\<^sub>i\<^sub>g"
   proof (insert assms, induct n arbitrary: \<S>\<^sub>2)
     case 0
     then have *: "\<S>\<^sub>1 \<hookrightarrow>\<^bsup>0\<^esup> \<S>\<^sub>2 \<Longrightarrow> \<S>\<^sub>1 = \<S>\<^sub>2"
@@ -186,26 +139,27 @@ theorem soundness_generalized:
       proof -
       fix n :: nat
       assume ff: "\<S>\<^sub>1 \<hookrightarrow>\<^bsup>Suc n\<^esup> \<S>\<^sub>2"
-      assume hi: "\<And>\<S>\<^sub>2. \<S>\<^sub>1 \<hookrightarrow>\<^bsup>n\<^esup> \<S>\<^sub>2 \<Longrightarrow> \<lbrakk> \<S>\<^sub>2 \<rbrakk>\<^sub>c\<^sub>o\<^sub>n\<^sub>f \<subseteq> \<lbrakk> \<S>\<^sub>1 \<rbrakk>\<^sub>c\<^sub>o\<^sub>n\<^sub>f"
+      assume hi: "\<And>\<S>\<^sub>2. \<S>\<^sub>1 \<hookrightarrow>\<^bsup>n\<^esup> \<S>\<^sub>2 \<Longrightarrow> \<lbrakk> \<S>\<^sub>2 \<rbrakk>\<^sub>c\<^sub>o\<^sub>n\<^sub>f\<^sub>i\<^sub>g \<subseteq> \<lbrakk> \<S>\<^sub>1 \<rbrakk>\<^sub>c\<^sub>o\<^sub>n\<^sub>f\<^sub>i\<^sub>g"
       obtain \<S>\<^sub>n where red_decomp: "\<S>\<^sub>1 \<hookrightarrow>\<^bsup>n\<^esup> \<S>\<^sub>n \<and> \<S>\<^sub>n \<hookrightarrow> \<S>\<^sub>2"
         using ff by auto
-      then have "\<lbrakk> \<S>\<^sub>1 \<rbrakk>\<^sub>c\<^sub>o\<^sub>n\<^sub>f \<supseteq> \<lbrakk> \<S>\<^sub>n \<rbrakk>\<^sub>c\<^sub>o\<^sub>n\<^sub>f"
+      then have "\<lbrakk> \<S>\<^sub>1 \<rbrakk>\<^sub>c\<^sub>o\<^sub>n\<^sub>f\<^sub>i\<^sub>g \<supseteq> \<lbrakk> \<S>\<^sub>n \<rbrakk>\<^sub>c\<^sub>o\<^sub>n\<^sub>f\<^sub>i\<^sub>g"
         using hi by (metis (no_types, lifting) ff relpowp_Suc_E someI_ex)
-      also have "\<lbrakk> \<S>\<^sub>n \<rbrakk>\<^sub>c\<^sub>o\<^sub>n\<^sub>f \<supseteq> \<lbrakk> \<S>\<^sub>2 \<rbrakk>\<^sub>c\<^sub>o\<^sub>n\<^sub>f"
+      also have "\<lbrakk> \<S>\<^sub>n \<rbrakk>\<^sub>c\<^sub>o\<^sub>n\<^sub>f\<^sub>i\<^sub>g \<supseteq> \<lbrakk> \<S>\<^sub>2 \<rbrakk>\<^sub>c\<^sub>o\<^sub>n\<^sub>f\<^sub>i\<^sub>g"
         by (simp add: red_decomp soundness')
-      ultimately show "\<lbrakk> \<S>\<^sub>1 \<rbrakk>\<^sub>c\<^sub>o\<^sub>n\<^sub>f \<supseteq> \<lbrakk> \<S>\<^sub>2 \<rbrakk>\<^sub>c\<^sub>o\<^sub>n\<^sub>f"
+      ultimately show "\<lbrakk> \<S>\<^sub>1 \<rbrakk>\<^sub>c\<^sub>o\<^sub>n\<^sub>f\<^sub>i\<^sub>g \<supseteq> \<lbrakk> \<S>\<^sub>2 \<rbrakk>\<^sub>c\<^sub>o\<^sub>n\<^sub>f\<^sub>i\<^sub>g"
         by auto
       qed
   qed
 
-(**) section \<open>Completeness\<close> (**)
+section \<open>Completeness\<close>
 
 theorem completeness:
-  shows "\<lbrakk> \<Gamma>, n \<turnstile> \<Psi> \<triangleright> \<Phi> \<rbrakk>\<^sub>c\<^sub>o\<^sub>n\<^sub>f \<subseteq> (\<Union>X\<in>\<F>\<^sub>n\<^sub>e\<^sub>x\<^sub>t (\<Gamma>, n \<turnstile> \<Psi> \<triangleright> \<Phi>). \<lbrakk> X \<rbrakk>\<^sub>c\<^sub>o\<^sub>n\<^sub>f)"
+  shows "\<lbrakk> \<Gamma>, n \<turnstile> \<Psi> \<triangleright> \<Phi> \<rbrakk>\<^sub>c\<^sub>o\<^sub>n\<^sub>f\<^sub>i\<^sub>g \<subseteq> (\<Union>X\<in>\<F>\<^sub>n\<^sub>e\<^sub>x\<^sub>t (\<Gamma>, n \<turnstile> \<Psi> \<triangleright> \<Phi>). \<lbrakk> X \<rbrakk>\<^sub>c\<^sub>o\<^sub>n\<^sub>f\<^sub>i\<^sub>g)"
   proof (induct \<Psi>)
     case Nil
     show ?case
-      using HeronConf_interp_at_index_instant_cases operational_semantics_step.instant_i by fastforce
+      using HeronConf_interp_at_index_instant_cases operational_semantics_step.simps operational_semantics_intro.instant_i
+      by fastforce
   next
     case (Cons \<psi> \<Psi>)
     then show ?case
@@ -213,107 +167,205 @@ theorem completeness:
         case (Sporadic K \<tau>)
         then show ?case
           using HeronConf_interp_at_index_sporadic_cases Fnext_solve_sporadic
-          by (smt UN_iff UnE mem_Collect_eq operational_semantics_step.sporadic_e1 operational_semantics_step.sporadic_e2 subsetI)
+          by (smt UN_iff UnE insert_subset subsetI)
       next
         case (SporadicOn K1 \<tau> K2)
         then show ?case 
-          using HeronConf_interp_at_index_sporadicon_cases Fnext_solve_sporadicon 
-          by (smt UN_iff UnE mem_Collect_eq operational_semantics_step.sporadic_on_e1 operational_semantics_step.sporadic_on_e2 subsetI)
+          using HeronConf_interp_at_index_sporadicon_cases Fnext_solve_sporadicon
+          by (smt UN_iff UnE insert_subset subsetI)
       next
         case (TagRelation K1 \<alpha> K2 \<beta>)
         then show ?case
           using HeronConf_interp_at_index_tagrel_cases Fnext_solve_tagrel
-          by (smt Sup_upper image_iff mem_Collect_eq operational_semantics_step.tagrel_e)
+          by (smt UN_iff UnE insert_subset subsetI)
       next
         case (Implies K1 K2)
         then show ?case
           using HeronConf_interp_at_index_implies_cases Fnext_solve_implies
-          by (smt UN_iff UnE mem_Collect_eq operational_semantics_step.implies_e1 operational_semantics_step.implies_e2 subsetI)
+          by (smt UN_iff UnE insert_subset subsetI)
       next
         case (TimeDelayedBy Kmast \<tau> Kmeas Kslave)
         then show ?case
           using HeronConf_interp_at_index_timedelayed_cases Fnext_solve_timedelayed
-          by (smt UN_iff UnE mem_Collect_eq operational_semantics_step.timedelayed_e1 operational_semantics_step.timedelayed_e2 subsetI)
+          by (smt UN_iff UnE insert_subset subsetI)
       qed
   qed
 
 theorem completeness':
-  shows "\<lbrakk> \<C> \<rbrakk>\<^sub>c\<^sub>o\<^sub>n\<^sub>f \<subseteq> (\<Union>X\<in>\<F>\<^sub>n\<^sub>e\<^sub>x\<^sub>t \<C>. \<lbrakk> X \<rbrakk>\<^sub>c\<^sub>o\<^sub>n\<^sub>f)"
+  shows "\<lbrakk> \<S> \<rbrakk>\<^sub>c\<^sub>o\<^sub>n\<^sub>f\<^sub>i\<^sub>g \<subseteq> (\<Union>X\<in>\<F>\<^sub>n\<^sub>e\<^sub>x\<^sub>t \<S>. \<lbrakk> X \<rbrakk>\<^sub>c\<^sub>o\<^sub>n\<^sub>f\<^sub>i\<^sub>g)"
   by (metis HeronConf_interpretation.cases completeness)
 
-(**) section \<open>Termination of instantaneous formulae elimination\<close> (**)
-(* Idea: A bounded monotonic sequence is convergent *)
-primrec measure_interpretation :: "TESL_formula \<Rightarrow> nat" ("\<lbrakk>\<lbrakk> _ \<rbrakk>\<rbrakk>\<^sub>m\<^sub>e\<^sub>a\<^sub>s") where
-    "\<lbrakk>\<lbrakk> [] \<rbrakk>\<rbrakk>\<^sub>m\<^sub>e\<^sub>a\<^sub>s = (0::nat)"
-  | "\<lbrakk>\<lbrakk> \<phi> # \<Phi> \<rbrakk>\<rbrakk>\<^sub>m\<^sub>e\<^sub>a\<^sub>s = (case \<phi> of
-                        _ sporadic _ on _ \<Rightarrow> 1 + \<lbrakk>\<lbrakk> \<Phi> \<rbrakk>\<rbrakk>\<^sub>m\<^sub>e\<^sub>a\<^sub>s
-                      | _                 \<Rightarrow> 2 + \<lbrakk>\<lbrakk> \<Phi> \<rbrakk>\<rbrakk>\<^sub>m\<^sub>e\<^sub>a\<^sub>s)"
+(*
+theorem completeness'':
+  assumes "\<rho> \<in> \<lbrakk> \<Gamma>\<^sub>1, n\<^sub>1 \<turnstile> \<Psi>\<^sub>1 \<triangleright> \<Phi>\<^sub>1 \<rbrakk>\<^sub>c\<^sub>o\<^sub>n\<^sub>f\<^sub>i\<^sub>g"
+  shows "\<exists>\<Gamma>\<^sub>2 n\<^sub>2 \<Psi>\<^sub>2 \<Phi>\<^sub>2. \<Gamma>\<^sub>1, n\<^sub>1 \<turnstile> \<Psi>\<^sub>1 \<triangleright> \<Phi>\<^sub>1 \<hookrightarrow> \<Gamma>\<^sub>2, n\<^sub>2 \<turnstile> \<Psi>\<^sub>2 \<triangleright> \<Phi>\<^sub>2
+           \<and> \<rho> \<in> \<lbrakk> \<Gamma>\<^sub>2, n\<^sub>2 \<turnstile> \<Psi>\<^sub>2 \<triangleright> \<Phi>\<^sub>2 \<rbrakk>\<^sub>c\<^sub>o\<^sub>n\<^sub>f\<^sub>i\<^sub>g"
+  proof (insert assms, induct \<Psi>\<^sub>1)
+    case Nil
+    have "\<rho> \<in> \<lbrakk> \<Gamma>\<^sub>1, Suc n\<^sub>1 \<turnstile> \<Phi>\<^sub>1 \<triangleright> [] \<rbrakk>\<^sub>c\<^sub>o\<^sub>n\<^sub>f\<^sub>i\<^sub>g"
+      using assms HeronConf_interp_at_index_instant_cases by auto
+    moreover have "\<Gamma>\<^sub>1, n\<^sub>1 \<turnstile> [] \<triangleright> \<Phi>\<^sub>1 \<hookrightarrow> \<Gamma>\<^sub>1, Suc n\<^sub>1 \<turnstile> \<Phi>\<^sub>1 \<triangleright> []"
+      using intro_part operational_semantics_intro.instant_i by auto
+    ultimately show ?case by blast
+  next
+    case (Cons \<psi>\<^sub>1 \<Psi>\<^sub>1)
+    then show ?case
+      proof (induct \<psi>\<^sub>1)
+        case (Sporadic x1 x2)
+        then show ?case
+          using HeronConf_interp_at_index_sporadic_cases
+          by (metis UnE elims_part sporadic_e1 sporadic_e2)
+      next
+        case (SporadicOn x1 x2 x3)
+        then show ?case
+          using HeronConf_interp_at_index_sporadicon_cases
+          by (metis UnE elims_part sporadic_on_e1 sporadic_on_e2)
+      next
+        case (TagRelation x1 x2 x3 x4)
+        then show ?case
+          using HeronConf_interp_at_index_tagrel_cases
+          by (metis elims_part tagrel_e)
+      next
+        case (Implies x1 x2)
+        then show ?case
+          using HeronConf_interp_at_index_implies_cases
+          by (metis UnE elims_part implies_e1 implies_e2)
+      next
+        case (TimeDelayedBy x1 x2 x3 x4)
+        then show ?case
+          using HeronConf_interp_at_index_timedelayed_cases
+          by (metis UnE elims_part timedelayed_e1 timedelayed_e2)
+      qed
+  qed
+*)
 
-fun measure_interpretation_config :: "config \<Rightarrow> nat" ("\<lbrakk>\<lbrakk> _ \<rbrakk>\<rbrakk>\<^sub>m\<^sub>e\<^sub>a\<^sub>s\<^sub>c\<^sub>o\<^sub>n\<^sub>f\<^sub>i\<^sub>g") where
-    "\<lbrakk>\<lbrakk> \<Gamma>, n \<turnstile> \<Psi> \<triangleright> \<Phi> \<rbrakk>\<rbrakk>\<^sub>m\<^sub>e\<^sub>a\<^sub>s\<^sub>c\<^sub>o\<^sub>n\<^sub>f\<^sub>i\<^sub>g = \<lbrakk>\<lbrakk> \<Psi> \<rbrakk>\<rbrakk>\<^sub>m\<^sub>e\<^sub>a\<^sub>s"
+theorem completeness''':
+  assumes "\<rho> \<in> \<lbrakk> \<S>\<^sub>1 \<rbrakk>\<^sub>c\<^sub>o\<^sub>n\<^sub>f\<^sub>i\<^sub>g"
+  shows "\<exists>\<S>\<^sub>2. \<S>\<^sub>1 \<hookrightarrow> \<S>\<^sub>2 \<and> \<rho> \<in> \<lbrakk> \<S>\<^sub>2 \<rbrakk>\<^sub>c\<^sub>o\<^sub>n\<^sub>f\<^sub>i\<^sub>g"
+  by (metis (mono_tags, lifting) UN_iff assms completeness' mem_Collect_eq set_rev_mp)
+
+theorem completeness'''':
+  assumes "\<rho> \<in> \<lbrakk> [], 0 \<turnstile> \<Psi> \<triangleright> [] \<rbrakk>\<^sub>c\<^sub>o\<^sub>n\<^sub>f\<^sub>i\<^sub>g"
+  shows "\<exists>\<S>. [], 0 \<turnstile> \<Psi> \<triangleright> [] \<hookrightarrow>\<^bsup>n\<^esup> \<S> \<and> \<rho> \<in> \<lbrakk> \<S> \<rbrakk>\<^sub>c\<^sub>o\<^sub>n\<^sub>f\<^sub>i\<^sub>g"
+  sorry
+
+section \<open>Termination of instant computation\<close>
+
+(* Idea: A bounded monotonic sequence is convergent *)
+primrec measure_interpretation :: "TESL_formula \<Rightarrow> nat" ("\<mu>") where
+    "\<mu> [] = (0::nat)"
+  | "\<mu> (\<phi> # \<Phi>) = (case \<phi> of
+                        _ sporadic _ on _ \<Rightarrow> 1 + \<mu> \<Phi>
+                      | _                 \<Rightarrow> 2 + \<mu> \<Phi>)"
+
+fun measure_interpretation_config :: "config \<Rightarrow> nat" ("\<mu>\<^sub>c\<^sub>o\<^sub>n\<^sub>f\<^sub>i\<^sub>g") where
+    "\<mu>\<^sub>c\<^sub>o\<^sub>n\<^sub>f\<^sub>i\<^sub>g (\<Gamma>, n \<turnstile> \<Psi> \<triangleright> \<Phi>) = \<mu> \<Psi>"
 
 lemma elimation_rules_strictly_decreasing:
   assumes "\<Gamma>\<^sub>1, n\<^sub>1 \<turnstile> \<Psi>\<^sub>1 \<triangleright> \<Phi>\<^sub>1  \<hookrightarrow>\<^sub>e  \<Gamma>\<^sub>2, n\<^sub>2 \<turnstile> \<Psi>\<^sub>2 \<triangleright> \<Phi>\<^sub>2"
-  shows "\<lbrakk>\<lbrakk> \<Psi>\<^sub>1 \<rbrakk>\<rbrakk>\<^sub>m\<^sub>e\<^sub>a\<^sub>s > \<lbrakk>\<lbrakk> \<Psi>\<^sub>2 \<rbrakk>\<rbrakk>\<^sub>m\<^sub>e\<^sub>a\<^sub>s"
+  shows "\<mu> \<Psi>\<^sub>1 > \<mu> \<Psi>\<^sub>2"
   by (insert assms, erule operational_semantics_elim.cases, auto)
 
 lemma elimation_rules_strictly_decreasing_meas:
   assumes "\<Gamma>\<^sub>1, n\<^sub>1 \<turnstile> \<Psi>\<^sub>1 \<triangleright> \<Phi>\<^sub>1  \<hookrightarrow>\<^sub>e  \<Gamma>\<^sub>2, n\<^sub>2 \<turnstile> \<Psi>\<^sub>2 \<triangleright> \<Phi>\<^sub>2"
-  shows "(\<Psi>\<^sub>2, \<Psi>\<^sub>1) \<in> measure measure_interpretation"
+  shows "(\<Psi>\<^sub>2, \<Psi>\<^sub>1) \<in> measure \<mu>"
   by (insert assms, erule operational_semantics_elim.cases, auto)
 
 lemma elimation_rules_strictly_decreasing_meas':
   assumes "\<S>\<^sub>1  \<hookrightarrow>\<^sub>e  \<S>\<^sub>2"
-  shows "(\<S>\<^sub>2, \<S>\<^sub>1) \<in> measure measure_interpretation_config"
-  sorry
+  shows "(\<S>\<^sub>2, \<S>\<^sub>1) \<in> measure \<mu>\<^sub>c\<^sub>o\<^sub>n\<^sub>f\<^sub>i\<^sub>g"
+  using elimation_rules_strictly_decreasing_meas
+  by (metis assms in_measure measure_interpretation_config.elims)
 
-lemma instant_computation_termination:
-  shows "wf {(\<S>\<^sub>1, \<S>\<^sub>2). \<S>\<^sub>1 \<hookrightarrow>\<^sub>e \<S>\<^sub>2}"
-  apply (rule wf_subset)
-  proof -
-    have "measure (\<lambda>\<S>. \<lbrakk>\<lbrakk> \<S> \<rbrakk>\<rbrakk>\<^sub>m\<^sub>e\<^sub>a\<^sub>s\<^sub>c\<^sub>o\<^sub>n\<^sub>f\<^sub>i\<^sub>g) = { (\<S>\<^sub>1, \<S>\<^sub>2). \<lbrakk>\<lbrakk> \<S>\<^sub>1 \<rbrakk>\<rbrakk>\<^sub>m\<^sub>e\<^sub>a\<^sub>s\<^sub>c\<^sub>o\<^sub>n\<^sub>f\<^sub>i\<^sub>g < \<lbrakk>\<lbrakk> \<S>\<^sub>2 \<rbrakk>\<rbrakk>\<^sub>m\<^sub>e\<^sub>a\<^sub>s\<^sub>c\<^sub>o\<^sub>n\<^sub>f\<^sub>i\<^sub>g }"
-      by (simp add: inv_image_def less_eq measure_def)
-    show "{(\<S>\<^sub>1, \<S>\<^sub>2). \<S>\<^sub>1 \<hookrightarrow>\<^sub>e \<S>\<^sub>2} \<subseteq> (measure (\<lambda>\<S>. \<lbrakk>\<lbrakk> \<S> \<rbrakk>\<rbrakk>\<^sub>m\<^sub>e\<^sub>a\<^sub>s\<^sub>c\<^sub>o\<^sub>n\<^sub>f\<^sub>i\<^sub>g))"
-      sorry  (* Pas dans le bon sens !?! *)
-    show "wf (measure measure_interpretation_config)"
-      by simp
+theorem instant_computation_termination:
+  shows "wfP (\<lambda>\<S>\<^sub>1 \<S>\<^sub>2. \<S>\<^sub>1 \<hookrightarrow>\<^sub>e\<^sup>\<leftarrow> \<S>\<^sub>2)"
+  proof (simp add: wfP_def)
+    show "wf {(\<S>\<^sub>1, \<S>\<^sub>2). \<S>\<^sub>1 \<hookrightarrow>\<^sub>e\<^sup>\<leftarrow> \<S>\<^sub>2}"
+    apply (rule wf_subset)
+    proof -
+      have "measure \<mu>\<^sub>c\<^sub>o\<^sub>n\<^sub>f\<^sub>i\<^sub>g = { (\<S>\<^sub>2, \<S>\<^sub>1). \<mu>\<^sub>c\<^sub>o\<^sub>n\<^sub>f\<^sub>i\<^sub>g \<S>\<^sub>2 < \<mu>\<^sub>c\<^sub>o\<^sub>n\<^sub>f\<^sub>i\<^sub>g \<S>\<^sub>1 }"
+        by (simp add: inv_image_def less_eq measure_def)
+      then show "{(\<S>\<^sub>1, \<S>\<^sub>2). \<S>\<^sub>1 \<hookrightarrow>\<^sub>e\<^sup>\<leftarrow> \<S>\<^sub>2} \<subseteq> (measure \<mu>\<^sub>c\<^sub>o\<^sub>n\<^sub>f\<^sub>i\<^sub>g)"
+        using elimation_rules_strictly_decreasing_meas' operational_semantics_elim_inv_def by auto
+      show "wf (measure measure_interpretation_config)"
+        by simp
+    qed
   qed
 
-theorem instant_computation_termination':
-  shows "wfP (\<lambda>\<S>\<^sub>1 \<S>\<^sub>2. \<S>\<^sub>1 \<hookrightarrow>\<^sub>e \<S>\<^sub>2)"
-  using instant_computation_termination
-  by (simp add: wfP_def)
+section \<open>Progress\<close>
 
-lemma run_index_progress:
+lemma run_index_increase:
   assumes "\<Gamma>\<^sub>1, n\<^sub>1 \<turnstile> \<Psi>\<^sub>1 \<triangleright> \<Phi>\<^sub>1  \<hookrightarrow>  \<Gamma>\<^sub>2, n\<^sub>2 \<turnstile> \<Psi>\<^sub>2 \<triangleright> \<Phi>\<^sub>2"
   shows "n\<^sub>2 = Suc n\<^sub>1 \<or> n\<^sub>2 = n\<^sub>1"
-  by (insert assms, erule operational_semantics_step.cases, auto)
+  apply (insert assms, erule operational_semantics_step.cases)
+  proof -
+  show "\<And>\<Gamma>\<^sub>1' n\<^sub>1' \<Psi>\<^sub>1' \<Phi>\<^sub>1' \<Gamma>\<^sub>2' n\<^sub>2' \<Psi>\<^sub>2' \<Phi>\<^sub>2'.
+       \<Gamma>\<^sub>1, n\<^sub>1 \<turnstile> \<Psi>\<^sub>1 \<triangleright> \<Phi>\<^sub>1 = \<Gamma>\<^sub>1', n\<^sub>1' \<turnstile> \<Psi>\<^sub>1' \<triangleright> \<Phi>\<^sub>1' \<Longrightarrow>
+       \<Gamma>\<^sub>2, n\<^sub>2 \<turnstile> \<Psi>\<^sub>2 \<triangleright> \<Phi>\<^sub>2 = \<Gamma>\<^sub>2', n\<^sub>2' \<turnstile> \<Psi>\<^sub>2' \<triangleright> \<Phi>\<^sub>2' \<Longrightarrow>
+       \<Gamma>\<^sub>1', n\<^sub>1' \<turnstile> \<Psi>\<^sub>1' \<triangleright> \<Phi>\<^sub>1' \<hookrightarrow>\<^sub>i \<Gamma>\<^sub>2', n\<^sub>2' \<turnstile> \<Psi>\<^sub>2' \<triangleright> \<Phi>\<^sub>2' \<Longrightarrow> n\<^sub>2 = Suc n\<^sub>1 \<or> n\<^sub>2 = n\<^sub>1"
+    by (simp add: operational_semantics_intro.simps)
+  show "\<And>\<Gamma>\<^sub>1' n\<^sub>1' \<Psi>\<^sub>1' \<Phi>\<^sub>1' \<Gamma>\<^sub>2' n\<^sub>2' \<Psi>\<^sub>2' \<Phi>\<^sub>2'.
+       \<Gamma>\<^sub>1, n\<^sub>1 \<turnstile> \<Psi>\<^sub>1 \<triangleright> \<Phi>\<^sub>1 = \<Gamma>\<^sub>1', n\<^sub>1' \<turnstile> \<Psi>\<^sub>1' \<triangleright> \<Phi>\<^sub>1' \<Longrightarrow>
+       \<Gamma>\<^sub>2, n\<^sub>2 \<turnstile> \<Psi>\<^sub>2 \<triangleright> \<Phi>\<^sub>2 = \<Gamma>\<^sub>2', n\<^sub>2' \<turnstile> \<Psi>\<^sub>2' \<triangleright> \<Phi>\<^sub>2' \<Longrightarrow>
+       \<Gamma>\<^sub>1', n\<^sub>1' \<turnstile> \<Psi>\<^sub>1' \<triangleright> \<Phi>\<^sub>1' \<hookrightarrow>\<^sub>e \<Gamma>\<^sub>2', n\<^sub>2' \<turnstile> \<Psi>\<^sub>2' \<triangleright> \<Phi>\<^sub>2' \<Longrightarrow> n\<^sub>2 = Suc n\<^sub>1 \<or> n\<^sub>2 = n\<^sub>1"
+    using operational_semantics_elim.simps by auto
+  qed
 
+lemma progress:
+  shows "\<exists>\<Gamma>\<^sub>2 n\<^sub>2 \<Psi>\<^sub>2 \<Phi>\<^sub>2. \<Gamma>\<^sub>1, n\<^sub>1 \<turnstile> \<Psi>\<^sub>1 \<triangleright> \<Phi>\<^sub>1  \<hookrightarrow>  \<Gamma>\<^sub>2, n\<^sub>2 \<turnstile> \<Psi>\<^sub>2 \<triangleright> \<Phi>\<^sub>2"
+  proof (induct \<Psi>\<^sub>1)
+    case Nil
+    then show ?case
+      using intro_part operational_semantics_intro.instant_i by blast
+  next
+    case (Cons \<psi>\<^sub>1 \<Psi>\<^sub>1)
+    then show ?case
+      proof (induct \<psi>\<^sub>1)
+        case (Sporadic x1 x2)
+        then show ?case
+          using elims_part operational_semantics_elim.sporadic_e1 by blast
+      next
+        case (SporadicOn x1 x2 x3)
+        then show ?case
+          using elims_part operational_semantics_elim.sporadic_on_e1 by blast
+      next
+        case (TagRelation x1 x2 x3 x4)
+        then show ?case
+          using elims_part operational_semantics_elim.tagrel_e by blast
+      next
+        case (Implies x1 x2)
+        then show ?case
+          using elims_part operational_semantics_elim.implies_e1 by blast
+      next
+        case (TimeDelayedBy x1 x2 x3 x4)
+  then show ?case
+    using elims_part operational_semantics_elim.timedelayed_e1 by blast
+      qed
+  qed
+
+(* Elementaire, simple par définition de \<rightarrow>\<^sub>\<nabla> *)
 lemma run_index_progress_simlstep:
   assumes "\<Gamma>\<^sub>1, n\<^sub>1 \<turnstile> \<Psi>\<^sub>1 \<triangleright> \<Phi>\<^sub>1  \<hookrightarrow>\<^sub>\<nabla>  \<Gamma>\<^sub>2, n\<^sub>2 \<turnstile> \<Psi>\<^sub>2 \<triangleright> \<Phi>\<^sub>2"
   shows "n\<^sub>2 = Suc n\<^sub>1"
-  apply (insert assms)
-  sorry
+  using assms
+  by (simp add: operational_semantics_simlstep.simps)
 
 (**) section \<open>Composition\<close> (**)
 
 lemma composition:
-  shows "\<lbrakk> \<Gamma>\<^sub>1, n \<turnstile> \<Psi>\<^sub>1 \<triangleright> \<Phi>\<^sub>1 \<rbrakk>\<^sub>c\<^sub>o\<^sub>n\<^sub>f \<inter> \<lbrakk> \<Gamma>\<^sub>2, n \<turnstile> \<Psi>\<^sub>2 \<triangleright> \<Phi>\<^sub>2 \<rbrakk>\<^sub>c\<^sub>o\<^sub>n\<^sub>f
-         = \<lbrakk> \<Gamma>\<^sub>1 @ \<Gamma>\<^sub>2, n \<turnstile> \<Psi>\<^sub>1 @ \<Psi>\<^sub>2 \<triangleright> \<Phi>\<^sub>1 @ \<Phi>\<^sub>2 \<rbrakk>\<^sub>c\<^sub>o\<^sub>n\<^sub>f"
+  shows "\<lbrakk> \<Gamma>\<^sub>1, n \<turnstile> \<Psi>\<^sub>1 \<triangleright> \<Phi>\<^sub>1 \<rbrakk>\<^sub>c\<^sub>o\<^sub>n\<^sub>f\<^sub>i\<^sub>g \<inter> \<lbrakk> \<Gamma>\<^sub>2, n \<turnstile> \<Psi>\<^sub>2 \<triangleright> \<Phi>\<^sub>2 \<rbrakk>\<^sub>c\<^sub>o\<^sub>n\<^sub>f\<^sub>i\<^sub>g
+         = \<lbrakk> \<Gamma>\<^sub>1 @ \<Gamma>\<^sub>2, n \<turnstile> \<Psi>\<^sub>1 @ \<Psi>\<^sub>2 \<triangleright> \<Phi>\<^sub>1 @ \<Phi>\<^sub>2 \<rbrakk>\<^sub>c\<^sub>o\<^sub>n\<^sub>f\<^sub>i\<^sub>g"
   using TESL_interp_at_index_composition symrun_interp_expansion by auto
 
 (**) section \<open>Semidecidability\<close> (**)
 (* The set of runs hence becomes recursively countable due to the previous observations. *)
 
 (**) section \<open>Existence\<close> (**)
-fun tagrel_consistent :: "TESL_formula \<Rightarrow> bool" where
-  "tagrel_consistent \<Phi> = undefined"
-
 lemma existence:
   (* Assumption that the linear system made of tag relations is consistent *)
   assumes "tagrel_consistent \<Phi>"
   shows "\<exists>\<rho>. \<rho> \<in> \<lbrakk>\<lbrakk> \<Phi> \<rbrakk>\<rbrakk>\<^sub>T\<^sub>E\<^sub>S\<^sub>L"
-oops
-(* proof (induction \<Phi>) *)
+  oops
+  (* proof (induction \<Phi>) *)
 
 end
