Operational.thy
@@ -2,7 +2,6 @@ theory Operational
 imports
     "TESL"
     "Run"
-    "Denotational"
 
 begin
 text{* Operational steps *}
@@ -10,48 +9,6 @@ text{* Operational steps *}
 abbreviation uncurry_conf
   :: "system \<Rightarrow> instant_index \<Rightarrow> TESL_formula \<Rightarrow> TESL_formula \<Rightarrow> config" ("_, _ \<turnstile> _ \<triangleright> _" 80) where
   "\<Gamma>, n \<turnstile> \<Psi> \<triangleright> \<Phi> \<equiv> (\<Gamma>, n, \<Psi>, \<Phi>)"
-
-inductive operational_semantics_step :: "config \<Rightarrow> config \<Rightarrow> bool" ("_ \<hookrightarrow> _" 70) where
-  instant_i:
-  "(* consistent_run \<Gamma> \<Longrightarrow> *)
-   \<Gamma>, n \<turnstile> [] \<triangleright> \<Phi>
-     \<hookrightarrow>  \<Gamma>, Suc n \<turnstile> \<Phi> \<triangleright> []"
-| sporadic_e1:
-  "(* consistent_run \<Gamma> \<Longrightarrow> *)
-   \<Gamma>, n \<turnstile> (K sporadic \<tau>) # \<Psi> \<triangleright> \<Phi>
-     \<hookrightarrow>  \<Gamma>, n \<turnstile> \<Psi> \<triangleright> (K sporadic \<tau>) # \<Phi>"
-| sporadic_e2:
-  "(* consistent_run ((K \<Up> n) # (K \<Down> n @ \<lfloor>\<tau>\<rfloor>) # \<Gamma>) \<Longrightarrow> *)
-   \<Gamma>, n \<turnstile> (K sporadic \<tau>) # \<Psi> \<triangleright> \<Phi>
-     \<hookrightarrow>  K \<Up> n # K \<Down> n @ \<lfloor>\<tau>\<rfloor> # \<Gamma>, n \<turnstile> \<Psi> \<triangleright> \<Phi>"
-| sporadic_on_e1:
-  "(* consistent_run \<Gamma> \<Longrightarrow> *)
-   \<Gamma>, n \<turnstile> (K\<^sub>1 sporadic \<tau> on K\<^sub>2) # \<Psi> \<triangleright> \<Phi>
-     \<hookrightarrow>  \<Gamma>, n \<turnstile> \<Psi> \<triangleright> (K\<^sub>1 sporadic \<tau> on K\<^sub>2) # \<Phi>"
-| sporadic_on_e2:
-  "(* consistent_run ((K\<^sub>1 \<Up> n) # (K\<^sub>2 \<Down> n @ \<tau>) # \<Gamma>) \<Longrightarrow> *)
-   \<Gamma>, n \<turnstile> (K\<^sub>1 sporadic \<tau> on K\<^sub>2) # \<Psi> \<triangleright> \<Phi>
-     \<hookrightarrow>  K\<^sub>1 \<Up> n # K\<^sub>2 \<Down> n @ \<tau> # \<Gamma>, n \<turnstile> \<Psi> \<triangleright> \<Phi>"
-| tagrel_e:
-  "(* consistent_run ((\<tau>\<^sub>v\<^sub>a\<^sub>r(K\<^sub>1, n) \<doteq> \<alpha> * \<tau>\<^sub>v\<^sub>a\<^sub>r(K\<^sub>2, n) + \<beta>) # \<Gamma>) \<Longrightarrow> *)
-   \<Gamma>, n \<turnstile> (tag-relation K\<^sub>1 = \<alpha> * K\<^sub>2 + \<beta>) # \<Psi> \<triangleright> \<Phi>
-     \<hookrightarrow>  (\<tau>\<^sub>v\<^sub>a\<^sub>r(K\<^sub>1, n) \<doteq> \<alpha> * \<tau>\<^sub>v\<^sub>a\<^sub>r(K\<^sub>2, n) + \<beta>) # \<Gamma>, n \<turnstile> \<Psi> \<triangleright> (tag-relation K\<^sub>1 = \<alpha> * K\<^sub>2 + \<beta>) # \<Phi>"
-| implies_e1:
-  "(* consistent_run (K\<^sub>1 \<not>\<Up> n # \<Gamma>) \<Longrightarrow> *)
-   \<Gamma>, n \<turnstile> (K\<^sub>1 implies K\<^sub>2) # \<Psi> \<triangleright> \<Phi>
-     \<hookrightarrow>  K\<^sub>1 \<not>\<Up> n # \<Gamma>, n \<turnstile> \<Psi> \<triangleright> (K\<^sub>1 implies K\<^sub>2) # \<Phi>"
-| implies_e2:
-  "(* consistent_run ((K\<^sub>1 \<Up> n) # (K\<^sub>2 \<Up> n) # \<Gamma>) \<Longrightarrow> *)
-   \<Gamma>, n \<turnstile> (K\<^sub>1 implies K\<^sub>2) # \<Psi> \<triangleright> \<Phi>
-     \<hookrightarrow>  K\<^sub>1 \<Up> n # K\<^sub>2 \<Up> n # \<Gamma>, n \<turnstile> \<Psi> \<triangleright> (K\<^sub>1 implies K\<^sub>2) # \<Phi>"
-| timedelayed_e1:
-  "(* consistent_run (K\<^sub>1 \<not>\<Up> n # \<Gamma>) \<Longrightarrow> *)
-   \<Gamma>, n \<turnstile> (K\<^sub>1 time-delayed by \<delta>\<tau> on K\<^sub>2 implies K\<^sub>3) # \<Psi> \<triangleright> \<Phi>
-     \<hookrightarrow>  K\<^sub>1 \<not>\<Up> n # \<Gamma>, n \<turnstile> \<Psi> \<triangleright> (K\<^sub>1 time-delayed by \<delta>\<tau> on K\<^sub>2 implies K\<^sub>3) # \<Phi>"
-| timedelayed_e2:
-  "(* consistent_run (K\<^sub>1 \<Up> n # \<Gamma>) \<Longrightarrow> *)
-   \<Gamma>, n \<turnstile> (K\<^sub>1 time-delayed by \<delta>\<tau> on K\<^sub>2 implies K\<^sub>3) # \<Psi> \<triangleright> \<Phi>
-     \<hookrightarrow>  K\<^sub>1 \<Up> n # \<Gamma>, n \<turnstile> (K\<^sub>3 sporadic \<lfloor>\<tau>\<^sub>v\<^sub>a\<^sub>r(K\<^sub>2, n) \<oplus> \<delta>\<tau>\<rfloor> on K\<^sub>2) # \<Psi> \<triangleright> (K\<^sub>1 time-delayed by \<delta>\<tau> on K\<^sub>2 implies K\<^sub>3) # \<Phi>"
 
 inductive operational_semantics_intro :: "config \<Rightarrow> config \<Rightarrow> bool" ("_ \<hookrightarrow>\<^sub>i _" 70) where
   instant_i:
@@ -97,39 +54,34 @@ inductive operational_semantics_elim :: "config \<Rightarrow> config \<Rightarro
    \<Gamma>, n \<turnstile> (K\<^sub>1 time-delayed by \<delta>\<tau> on K\<^sub>2 implies K\<^sub>3) # \<Psi> \<triangleright> \<Phi>
      \<hookrightarrow>\<^sub>e  K\<^sub>1 \<Up> n # \<Gamma>, n \<turnstile> (K\<^sub>3 sporadic \<lfloor>\<tau>\<^sub>v\<^sub>a\<^sub>r(K\<^sub>2, n) \<oplus> \<delta>\<tau>\<rfloor> on K\<^sub>2) # \<Psi> \<triangleright> (K\<^sub>1 time-delayed by \<delta>\<tau> on K\<^sub>2 implies K\<^sub>3) # \<Phi>"
 
-find_theorems name:"operational_semantics_step"
-
-lemma operational_semantics_split:
-  shows "\<S>\<^sub>1 \<hookrightarrow> \<S>\<^sub>2 = \<S>\<^sub>1 \<hookrightarrow>\<^sub>i \<S>\<^sub>2 \<or> \<S>\<^sub>1 \<hookrightarrow>\<^sub>e \<S>\<^sub>2"
-  apply (rule operational_semantics_step.induct)
-  defer
-  apply (simp add: operational_semantics_intro.instant_i operational_semantics_step.instant_i)
-  apply (simp add: operational_semantics_elim.sporadic_e1)
-  apply (simp add: operational_semantics_elim.sporadic_e2)
-  apply (simp add: operational_semantics_elim.sporadic_on_e1)
-  apply (simp add: operational_semantics_elim.sporadic_on_e2)
-  apply (simp add: operational_semantics_elim.tagrel_e)
-  apply (simp add: operational_semantics_elim.implies_e1)
-  apply (simp add: operational_semantics_elim.implies_e2)
-  apply (simp add: operational_semantics_elim.timedelayed_e1)
-  apply (simp add: operational_semantics_elim.timedelayed_e2)
-  sorry
+inductive operational_semantics_step :: "config \<Rightarrow> config \<Rightarrow> bool" ("_ \<hookrightarrow> _" 70) where
+    intro_part: "\<Gamma>\<^sub>1, n\<^sub>1 \<turnstile> \<Psi>\<^sub>1 \<triangleright> \<Phi>\<^sub>1  \<hookrightarrow>\<^sub>i  \<Gamma>\<^sub>2, n\<^sub>2 \<turnstile> \<Psi>\<^sub>2 \<triangleright> \<Phi>\<^sub>2
+   \<Longrightarrow> \<Gamma>\<^sub>1, n\<^sub>1 \<turnstile> \<Psi>\<^sub>1 \<triangleright> \<Phi>\<^sub>1  \<hookrightarrow>  \<Gamma>\<^sub>2, n\<^sub>2 \<turnstile> \<Psi>\<^sub>2 \<triangleright> \<Phi>\<^sub>2"
+  | elims_part: "\<Gamma>\<^sub>1, n\<^sub>1 \<turnstile> \<Psi>\<^sub>1 \<triangleright> \<Phi>\<^sub>1  \<hookrightarrow>\<^sub>e  \<Gamma>\<^sub>2, n\<^sub>2 \<turnstile> \<Psi>\<^sub>2 \<triangleright> \<Phi>\<^sub>2
+   \<Longrightarrow> \<Gamma>\<^sub>1, n\<^sub>1 \<turnstile> \<Psi>\<^sub>1 \<triangleright> \<Phi>\<^sub>1  \<hookrightarrow>  \<Gamma>\<^sub>2, n\<^sub>2 \<turnstile> \<Psi>\<^sub>2 \<triangleright> \<Phi>\<^sub>2"
 
 abbreviation operational_semantics_step_rtranclp :: "config \<Rightarrow> config \<Rightarrow> bool" ("_ \<hookrightarrow>\<^sup>*\<^sup>* _" 70) where
-  "A \<hookrightarrow>\<^sup>*\<^sup>* B \<equiv> operational_semantics_step\<^sup>*\<^sup>* A B"
+  "\<C>\<^sub>1 \<hookrightarrow>\<^sup>*\<^sup>* \<C>\<^sub>2 \<equiv> operational_semantics_step\<^sup>*\<^sup>* \<C>\<^sub>1 \<C>\<^sub>2"
 
 abbreviation operational_semantics_step_tranclp :: "config \<Rightarrow> config \<Rightarrow> bool" ("_ \<hookrightarrow>\<^sup>+\<^sup>+ _" 70) where
-  "A \<hookrightarrow>\<^sup>+\<^sup>+ B \<equiv> operational_semantics_step\<^sup>+\<^sup>+ A B"
+  "\<C>\<^sub>1 \<hookrightarrow>\<^sup>+\<^sup>+ \<C>\<^sub>2 \<equiv> operational_semantics_step\<^sup>+\<^sup>+ \<C>\<^sub>1 \<C>\<^sub>2"
 
 abbreviation operational_semantics_step_reflclp :: "config \<Rightarrow> config \<Rightarrow> bool" ("_ \<hookrightarrow>\<^sup>=\<^sup>= _" 70) where
-  "A \<hookrightarrow>\<^sup>=\<^sup>= B \<equiv> operational_semantics_step\<^sup>=\<^sup>= A B"
+  "\<C>\<^sub>1 \<hookrightarrow>\<^sup>=\<^sup>= \<C>\<^sub>2 \<equiv> operational_semantics_step\<^sup>=\<^sup>= \<C>\<^sub>1 \<C>\<^sub>2"
 
 abbreviation operational_semantics_step_relpowp :: "config \<Rightarrow> nat \<Rightarrow> config \<Rightarrow> bool" ("_ \<hookrightarrow>\<^bsup>_\<^esup> _" 70) where
-  "A \<hookrightarrow>\<^bsup>n\<^esup> B \<equiv> (operational_semantics_step ^^ n) A B"
+  "\<C>\<^sub>1 \<hookrightarrow>\<^bsup>n\<^esup> \<C>\<^sub>2 \<equiv> (operational_semantics_step ^^ n) \<C>\<^sub>1 \<C>\<^sub>2"
 
+definition operational_semantics_elim_inv :: "config \<Rightarrow> config \<Rightarrow> bool" ("_ \<hookrightarrow>\<^sub>e\<^sup>\<leftarrow> _" 70) where
+  "\<C>\<^sub>1 \<hookrightarrow>\<^sub>e\<^sup>\<leftarrow> \<C>\<^sub>2 \<equiv> \<C>\<^sub>2 \<hookrightarrow>\<^sub>e \<C>\<^sub>1"
+
+(* TODO *)
 inductive operational_semantics_simlstep :: "config \<Rightarrow> config \<Rightarrow> bool" ("_ \<hookrightarrow>\<^sub>\<nabla> _" 70) where
   "(\<Gamma>\<^sub>1, n \<turnstile> [] \<triangleright> \<Phi>\<^sub>1) \<hookrightarrow>\<^sup>+\<^sup>+ (\<Gamma>, n + 1 \<turnstile> [] \<triangleright> \<Phi>\<^sub>2) \<Longrightarrow>
-   (\<Gamma>\<^sub>1, n \<turnstile> [] \<triangleright> \<Phi>\<^sub>1) \<hookrightarrow>\<^sub>\<nabla> (\<Gamma>, n + 1 \<turnstile> [] \<triangleright> \<Phi>\<^sub>2)"
+   \<Psi>\<^sub>1 = [] \<Longrightarrow>
+   \<Psi>\<^sub>2 = [] \<Longrightarrow>
+   n' = Suc n \<Longrightarrow>
+   (\<Gamma>\<^sub>1, n \<turnstile> \<Psi>\<^sub>1 \<triangleright> \<Phi>\<^sub>1) \<hookrightarrow>\<^sub>\<nabla> (\<Gamma>, n' \<turnstile> \<Psi>\<^sub>2 \<triangleright> \<Phi>\<^sub>2)"
 
 abbreviation Fnext_solve :: "config \<Rightarrow> config set" ("\<F>\<^sub>n\<^sub>e\<^sub>x\<^sub>t _") where
   "\<F>\<^sub>n\<^sub>e\<^sub>x\<^sub>t \<S> \<equiv> { \<S>'. \<S> \<hookrightarrow> \<S>' }"
@@ -137,166 +89,36 @@ abbreviation Fnext_solve :: "config \<Rightarrow> config set" ("\<F>\<^sub>n\<^s
 lemma Fnext_solve_instant:
   shows "\<F>\<^sub>n\<^sub>e\<^sub>x\<^sub>t (\<Gamma>, n \<turnstile> [] \<triangleright> \<Phi>)
           \<supseteq> { \<Gamma>, Suc n \<turnstile> \<Phi> \<triangleright> [] }"
-  by (simp add: operational_semantics_step.instant_i)
+  by (simp add: operational_semantics_step.simps operational_semantics_intro.instant_i)
 
 lemma Fnext_solve_sporadic:
   shows "\<F>\<^sub>n\<^sub>e\<^sub>x\<^sub>t (\<Gamma>, n \<turnstile> (K sporadic \<tau>) # \<Psi> \<triangleright> \<Phi>)
           \<supseteq> { \<Gamma>, n \<turnstile> \<Psi> \<triangleright> (K sporadic \<tau>) # \<Phi>,
               K \<Up> n # K \<Down> n @ \<lfloor>\<tau>\<rfloor> # \<Gamma>, n \<turnstile> \<Psi> \<triangleright> \<Phi> }"
-  by (simp add: operational_semantics_step.sporadic_e1 operational_semantics_step.sporadic_e2)
+  by (simp add: operational_semantics_step.simps operational_semantics_elim.sporadic_e1 operational_semantics_elim.sporadic_e2)
 
 lemma Fnext_solve_sporadicon:
   shows "\<F>\<^sub>n\<^sub>e\<^sub>x\<^sub>t (\<Gamma>, n \<turnstile> (K\<^sub>1 sporadic \<tau> on K\<^sub>2) # \<Psi> \<triangleright> \<Phi>)
           \<supseteq> { \<Gamma>, n \<turnstile> \<Psi> \<triangleright> (K\<^sub>1 sporadic \<tau> on K\<^sub>2) # \<Phi>,
               K\<^sub>1 \<Up> n # K\<^sub>2 \<Down> n @ \<tau> # \<Gamma>, n \<turnstile> \<Psi> \<triangleright> \<Phi> }"
-  by (simp add: operational_semantics_step.sporadic_on_e1 operational_semantics_step.sporadic_on_e2)
+  by (simp add: operational_semantics_step.simps operational_semantics_elim.sporadic_on_e1 operational_semantics_elim.sporadic_on_e2)
 
 lemma Fnext_solve_tagrel:
   shows "\<F>\<^sub>n\<^sub>e\<^sub>x\<^sub>t (\<Gamma>, n \<turnstile> (tag-relation K\<^sub>1 = \<alpha> * K\<^sub>2 + \<beta>) # \<Psi> \<triangleright> \<Phi>)
           \<supseteq> { (\<tau>\<^sub>v\<^sub>a\<^sub>r(K\<^sub>1, n) \<doteq> \<alpha> * \<tau>\<^sub>v\<^sub>a\<^sub>r(K\<^sub>2, n) + \<beta>) # \<Gamma>, n \<turnstile> \<Psi> \<triangleright> (tag-relation K\<^sub>1 = \<alpha> * K\<^sub>2 + \<beta>) # \<Phi> }"
-  by (simp add: operational_semantics_step.tagrel_e)
+  by (simp add: operational_semantics_step.simps operational_semantics_elim.tagrel_e)
 
 lemma Fnext_solve_implies:
   shows "\<F>\<^sub>n\<^sub>e\<^sub>x\<^sub>t (\<Gamma>, n \<turnstile> (K\<^sub>1 implies K\<^sub>2) # \<Psi> \<triangleright> \<Phi>)
           \<supseteq> { K\<^sub>1 \<not>\<Up> n # \<Gamma>, n \<turnstile> \<Psi> \<triangleright> (K\<^sub>1 implies K\<^sub>2) # \<Phi>,
               K\<^sub>1 \<Up> n # K\<^sub>2 \<Up> n # \<Gamma>, n \<turnstile> \<Psi> \<triangleright> (K\<^sub>1 implies K\<^sub>2) # \<Phi>}"
-  by (simp add: operational_semantics_step.implies_e1 operational_semantics_step.implies_e2)
+  by (simp add: operational_semantics_step.simps operational_semantics_elim.implies_e1 operational_semantics_elim.implies_e2)
 
 lemma Fnext_solve_timedelayed:
   shows "\<F>\<^sub>n\<^sub>e\<^sub>x\<^sub>t (\<Gamma>, n \<turnstile> (K\<^sub>1 time-delayed by \<delta>\<tau> on K\<^sub>2 implies K\<^sub>3) # \<Psi> \<triangleright> \<Phi>)
           \<supseteq> { K\<^sub>1 \<not>\<Up> n # \<Gamma>, n \<turnstile> \<Psi> \<triangleright> (K\<^sub>1 time-delayed by \<delta>\<tau> on K\<^sub>2 implies K\<^sub>3) # \<Phi>,
               K\<^sub>1 \<Up> n # \<Gamma>, n \<turnstile> (K\<^sub>3 sporadic \<lfloor>\<tau>\<^sub>v\<^sub>a\<^sub>r(K\<^sub>2, n) \<oplus> \<delta>\<tau>\<rfloor> on K\<^sub>2) # \<Psi> \<triangleright> (K\<^sub>1 time-delayed by \<delta>\<tau> on K\<^sub>2 implies K\<^sub>3) # \<Phi> }"
-  by (simp add: operational_semantics_step.timedelayed_e1 operational_semantics_step.timedelayed_e2)
-
-
-fun HeronConf_interpretation :: "config \<Rightarrow> run set" ("\<lbrakk> _ \<rbrakk>\<^sub>c\<^sub>o\<^sub>n\<^sub>f" 71) where
-  "\<lbrakk> \<Gamma>, n \<turnstile> \<Psi> \<triangleright> \<Phi> \<rbrakk>\<^sub>c\<^sub>o\<^sub>n\<^sub>f = \<lbrakk>\<lbrakk> \<Gamma> \<rbrakk>\<rbrakk>\<^sub>s\<^sub>y\<^sub>m\<^sub>r\<^sub>u\<^sub>n \<inter> \<lbrakk>\<lbrakk> \<Psi> \<nabla> n \<rbrakk>\<rbrakk>\<^sub>T\<^sub>E\<^sub>S\<^sub>L \<inter> \<lbrakk>\<lbrakk> \<Phi> \<nabla> Suc n \<rbrakk>\<rbrakk>\<^sub>T\<^sub>E\<^sub>S\<^sub>L"
-
-lemma HeronConf_interp_at_index_instant_cases:
-  shows "\<lbrakk> \<Gamma>, n \<turnstile> [] \<triangleright> \<Phi> \<rbrakk>\<^sub>c\<^sub>o\<^sub>n\<^sub>f
-          = \<lbrakk> \<Gamma>, Suc n \<turnstile> \<Phi> \<triangleright> [] \<rbrakk>\<^sub>c\<^sub>o\<^sub>n\<^sub>f"
-  proof -
-    have "\<lbrakk> \<Gamma>, n \<turnstile> [] \<triangleright> \<Phi> \<rbrakk>\<^sub>c\<^sub>o\<^sub>n\<^sub>f = \<lbrakk>\<lbrakk> \<Gamma> \<rbrakk>\<rbrakk>\<^sub>s\<^sub>y\<^sub>m\<^sub>r\<^sub>u\<^sub>n \<inter> \<lbrakk>\<lbrakk> [] \<nabla> n \<rbrakk>\<rbrakk>\<^sub>T\<^sub>E\<^sub>S\<^sub>L \<inter> \<lbrakk>\<lbrakk> \<Phi> \<nabla> Suc n \<rbrakk>\<rbrakk>\<^sub>T\<^sub>E\<^sub>S\<^sub>L"
-      by simp
-    moreover have "\<lbrakk> \<Gamma>, Suc n \<turnstile> \<Phi> \<triangleright> [] \<rbrakk>\<^sub>c\<^sub>o\<^sub>n\<^sub>f = \<lbrakk>\<lbrakk> \<Gamma> \<rbrakk>\<rbrakk>\<^sub>s\<^sub>y\<^sub>m\<^sub>r\<^sub>u\<^sub>n \<inter> \<lbrakk>\<lbrakk> \<Phi> \<nabla> Suc n \<rbrakk>\<rbrakk>\<^sub>T\<^sub>E\<^sub>S\<^sub>L \<inter> \<lbrakk>\<lbrakk> [] \<nabla> Suc n \<rbrakk>\<rbrakk>\<^sub>T\<^sub>E\<^sub>S\<^sub>L"
-      by simp
-    moreover have "\<lbrakk>\<lbrakk> \<Gamma> \<rbrakk>\<rbrakk>\<^sub>s\<^sub>y\<^sub>m\<^sub>r\<^sub>u\<^sub>n \<inter> \<lbrakk>\<lbrakk> [] \<nabla> n \<rbrakk>\<rbrakk>\<^sub>T\<^sub>E\<^sub>S\<^sub>L \<inter> \<lbrakk>\<lbrakk> \<Phi> \<nabla> Suc n \<rbrakk>\<rbrakk>\<^sub>T\<^sub>E\<^sub>S\<^sub>L
-                   = \<lbrakk>\<lbrakk> \<Gamma> \<rbrakk>\<rbrakk>\<^sub>s\<^sub>y\<^sub>m\<^sub>r\<^sub>u\<^sub>n \<inter> \<lbrakk>\<lbrakk> \<Phi> \<nabla> Suc n \<rbrakk>\<rbrakk>\<^sub>T\<^sub>E\<^sub>S\<^sub>L \<inter> \<lbrakk>\<lbrakk> [] \<nabla> Suc n \<rbrakk>\<rbrakk>\<^sub>T\<^sub>E\<^sub>S\<^sub>L"
-      by simp
-    ultimately show ?thesis by blast
-  qed
-
-lemma HeronConf_interp_at_index_sporadic_cases:
-  shows "\<lbrakk> \<Gamma>, n \<turnstile> (K sporadic \<tau>) # \<Psi> \<triangleright> \<Phi> \<rbrakk>\<^sub>c\<^sub>o\<^sub>n\<^sub>f
-          = \<lbrakk> \<Gamma>, n \<turnstile> \<Psi> \<triangleright> (K sporadic \<tau>) # \<Phi> \<rbrakk>\<^sub>c\<^sub>o\<^sub>n\<^sub>f
-          \<union> \<lbrakk> K \<Up> n # K \<Down> n @ \<lfloor>\<tau>\<rfloor> # \<Gamma>, n \<turnstile> \<Psi> \<triangleright> \<Phi> \<rbrakk>\<^sub>c\<^sub>o\<^sub>n\<^sub>f"
-  proof -
-    have "\<lbrakk> \<Gamma>, n \<turnstile> (K sporadic \<tau>) # \<Psi> \<triangleright> \<Phi> \<rbrakk>\<^sub>c\<^sub>o\<^sub>n\<^sub>f = \<lbrakk>\<lbrakk> \<Gamma> \<rbrakk>\<rbrakk>\<^sub>s\<^sub>y\<^sub>m\<^sub>r\<^sub>u\<^sub>n \<inter> \<lbrakk>\<lbrakk> (K sporadic \<tau>) # \<Psi> \<nabla> n \<rbrakk>\<rbrakk>\<^sub>T\<^sub>E\<^sub>S\<^sub>L \<inter> \<lbrakk>\<lbrakk> \<Phi> \<nabla> Suc n \<rbrakk>\<rbrakk>\<^sub>T\<^sub>E\<^sub>S\<^sub>L"
-      by simp
-    moreover have "\<lbrakk> \<Gamma>, n \<turnstile> \<Psi> \<triangleright> (K sporadic \<tau>) # \<Phi> \<rbrakk>\<^sub>c\<^sub>o\<^sub>n\<^sub>f = \<lbrakk>\<lbrakk> \<Gamma> \<rbrakk>\<rbrakk>\<^sub>s\<^sub>y\<^sub>m\<^sub>r\<^sub>u\<^sub>n \<inter> \<lbrakk>\<lbrakk> \<Psi> \<nabla> n \<rbrakk>\<rbrakk>\<^sub>T\<^sub>E\<^sub>S\<^sub>L \<inter> \<lbrakk>\<lbrakk> (K sporadic \<tau>) # \<Phi> \<nabla> Suc n \<rbrakk>\<rbrakk>\<^sub>T\<^sub>E\<^sub>S\<^sub>L"
-      by simp
-    moreover have "\<lbrakk> K \<Up> n # K \<Down> n @ \<lfloor>\<tau>\<rfloor> # \<Gamma>, n \<turnstile> \<Psi> \<triangleright> \<Phi> \<rbrakk>\<^sub>c\<^sub>o\<^sub>n\<^sub>f = \<lbrakk>\<lbrakk> K \<Up> n # K \<Down> n @ \<lfloor>\<tau>\<rfloor> # \<Gamma> \<rbrakk>\<rbrakk>\<^sub>s\<^sub>y\<^sub>m\<^sub>r\<^sub>u\<^sub>n \<inter> \<lbrakk>\<lbrakk> \<Psi> \<nabla> n \<rbrakk>\<rbrakk>\<^sub>T\<^sub>E\<^sub>S\<^sub>L \<inter> \<lbrakk>\<lbrakk> \<Phi> \<nabla> Suc n \<rbrakk>\<rbrakk>\<^sub>T\<^sub>E\<^sub>S\<^sub>L"
-      by simp
-    ultimately show ?thesis
-    proof -
-      have "(\<lbrakk> K \<Up> n \<rbrakk>\<^sub>s\<^sub>y\<^sub>m\<^sub>r\<^sub>u\<^sub>n \<inter> \<lbrakk> K \<Down> n @ \<lfloor> \<tau> \<rfloor> \<rbrakk>\<^sub>s\<^sub>y\<^sub>m\<^sub>r\<^sub>u\<^sub>n \<union> \<lbrakk> K sporadic \<tau> \<nabla> Suc n \<rbrakk>\<^sub>T\<^sub>E\<^sub>S\<^sub>L) \<inter> \<lbrakk>\<lbrakk> \<Psi> \<nabla> n \<rbrakk>\<rbrakk>\<^sub>T\<^sub>E\<^sub>S\<^sub>L = \<lbrakk>\<lbrakk> (K sporadic \<tau>) # \<Psi> \<nabla> n \<rbrakk>\<rbrakk>\<^sub>T\<^sub>E\<^sub>S\<^sub>L"
-        using TESL_interp_at_index_sporadic_cases TESL_interpretation_at_index_cons_morph by blast
-  then have "\<lbrakk> \<Gamma>, n \<turnstile> (K sporadic \<tau>) # \<Psi> \<triangleright> \<Phi> \<rbrakk>\<^sub>c\<^sub>o\<^sub>n\<^sub>f = (\<lbrakk>\<lbrakk> K \<Up> n # K \<Down> n @ \<lfloor> \<tau> \<rfloor> # \<Gamma> \<rbrakk>\<rbrakk>\<^sub>s\<^sub>y\<^sub>m\<^sub>r\<^sub>u\<^sub>n \<inter> \<lbrakk>\<lbrakk> \<Psi> \<nabla> n \<rbrakk>\<rbrakk>\<^sub>T\<^sub>E\<^sub>S\<^sub>L \<union> \<lbrakk>\<lbrakk> \<Gamma> \<rbrakk>\<rbrakk>\<^sub>s\<^sub>y\<^sub>m\<^sub>r\<^sub>u\<^sub>n \<inter> \<lbrakk>\<lbrakk> \<Psi> \<nabla> n \<rbrakk>\<rbrakk>\<^sub>T\<^sub>E\<^sub>S\<^sub>L \<inter> \<lbrakk> K sporadic \<tau> \<nabla> Suc n \<rbrakk>\<^sub>T\<^sub>E\<^sub>S\<^sub>L) \<inter> \<lbrakk>\<lbrakk> \<Phi> \<nabla> Suc n \<rbrakk>\<rbrakk>\<^sub>T\<^sub>E\<^sub>S\<^sub>L"
-    by auto
-      then show ?thesis
-        by (simp add: Int_Un_distrib2 Int_assoc Un_commute)
-    qed
-  qed
-
-lemma HeronConf_interp_at_index_sporadicon_cases:
-  shows "\<lbrakk> \<Gamma>, n \<turnstile> (K\<^sub>1 sporadic \<tau> on K\<^sub>2) # \<Psi> \<triangleright> \<Phi> \<rbrakk>\<^sub>c\<^sub>o\<^sub>n\<^sub>f
-          = \<lbrakk> \<Gamma>, n \<turnstile> \<Psi> \<triangleright> (K\<^sub>1 sporadic \<tau> on K\<^sub>2) # \<Phi> \<rbrakk>\<^sub>c\<^sub>o\<^sub>n\<^sub>f
-          \<union> \<lbrakk> K\<^sub>1 \<Up> n # K\<^sub>2 \<Down> n @ \<tau> # \<Gamma>, n \<turnstile> \<Psi> \<triangleright> \<Phi> \<rbrakk>\<^sub>c\<^sub>o\<^sub>n\<^sub>f"
-  proof -
-    have "\<lbrakk> \<Gamma>, n \<turnstile> (K\<^sub>1 sporadic \<tau> on K\<^sub>2) # \<Psi> \<triangleright> \<Phi> \<rbrakk>\<^sub>c\<^sub>o\<^sub>n\<^sub>f = \<lbrakk>\<lbrakk> \<Gamma> \<rbrakk>\<rbrakk>\<^sub>s\<^sub>y\<^sub>m\<^sub>r\<^sub>u\<^sub>n \<inter> \<lbrakk>\<lbrakk> (K\<^sub>1 sporadic \<tau> on K\<^sub>2) # \<Psi> \<nabla> n \<rbrakk>\<rbrakk>\<^sub>T\<^sub>E\<^sub>S\<^sub>L \<inter> \<lbrakk>\<lbrakk> \<Phi> \<nabla> Suc n \<rbrakk>\<rbrakk>\<^sub>T\<^sub>E\<^sub>S\<^sub>L"
-      by simp
-    moreover have "\<lbrakk> \<Gamma>, n \<turnstile> \<Psi> \<triangleright> (K\<^sub>1 sporadic \<tau> on K\<^sub>2) # \<Phi> \<rbrakk>\<^sub>c\<^sub>o\<^sub>n\<^sub>f = \<lbrakk>\<lbrakk> \<Gamma> \<rbrakk>\<rbrakk>\<^sub>s\<^sub>y\<^sub>m\<^sub>r\<^sub>u\<^sub>n \<inter> \<lbrakk>\<lbrakk> \<Psi> \<nabla> n \<rbrakk>\<rbrakk>\<^sub>T\<^sub>E\<^sub>S\<^sub>L \<inter> \<lbrakk>\<lbrakk> (K\<^sub>1 sporadic \<tau> on K\<^sub>2) # \<Phi> \<nabla> Suc n \<rbrakk>\<rbrakk>\<^sub>T\<^sub>E\<^sub>S\<^sub>L"
-      by simp
-    moreover have "\<lbrakk> K\<^sub>1 \<Up> n # K\<^sub>2 \<Down> n @ \<tau> # \<Gamma>, n \<turnstile> \<Psi> \<triangleright> \<Phi> \<rbrakk>\<^sub>c\<^sub>o\<^sub>n\<^sub>f = \<lbrakk>\<lbrakk> K\<^sub>1 \<Up> n # K\<^sub>2 \<Down> n @ \<tau> # \<Gamma> \<rbrakk>\<rbrakk>\<^sub>s\<^sub>y\<^sub>m\<^sub>r\<^sub>u\<^sub>n \<inter> \<lbrakk>\<lbrakk> \<Psi> \<nabla> n \<rbrakk>\<rbrakk>\<^sub>T\<^sub>E\<^sub>S\<^sub>L \<inter> \<lbrakk>\<lbrakk> \<Phi> \<nabla> Suc n \<rbrakk>\<rbrakk>\<^sub>T\<^sub>E\<^sub>S\<^sub>L"
-      by simp
-    ultimately show ?thesis
-    proof -
-      have "(\<lbrakk> K\<^sub>1 \<Up> n \<rbrakk>\<^sub>s\<^sub>y\<^sub>m\<^sub>r\<^sub>u\<^sub>n \<inter> \<lbrakk> K\<^sub>2 \<Down> n @ \<tau> \<rbrakk>\<^sub>s\<^sub>y\<^sub>m\<^sub>r\<^sub>u\<^sub>n \<union> \<lbrakk> K\<^sub>1 sporadic \<tau> on K\<^sub>2 \<nabla> Suc n \<rbrakk>\<^sub>T\<^sub>E\<^sub>S\<^sub>L) \<inter> (\<lbrakk>\<lbrakk> \<Gamma> \<rbrakk>\<rbrakk>\<^sub>s\<^sub>y\<^sub>m\<^sub>r\<^sub>u\<^sub>n \<inter> \<lbrakk>\<lbrakk> \<Psi> \<nabla> n \<rbrakk>\<rbrakk>\<^sub>T\<^sub>E\<^sub>S\<^sub>L) = \<lbrakk> K\<^sub>1 sporadic \<tau> on K\<^sub>2 \<nabla> n \<rbrakk>\<^sub>T\<^sub>E\<^sub>S\<^sub>L \<inter> (\<lbrakk>\<lbrakk> \<Psi> \<nabla> n \<rbrakk>\<rbrakk>\<^sub>T\<^sub>E\<^sub>S\<^sub>L \<inter> \<lbrakk>\<lbrakk> \<Gamma> \<rbrakk>\<rbrakk>\<^sub>s\<^sub>y\<^sub>m\<^sub>r\<^sub>u\<^sub>n)"
-        using TESL_interp_at_index_sporadicon_cases by blast
-      then have "\<lbrakk>\<lbrakk> K\<^sub>1 \<Up> n # K\<^sub>2 \<Down> n @ \<tau> # \<Gamma> \<rbrakk>\<rbrakk>\<^sub>s\<^sub>y\<^sub>m\<^sub>r\<^sub>u\<^sub>n \<inter> \<lbrakk>\<lbrakk> \<Psi> \<nabla> n \<rbrakk>\<rbrakk>\<^sub>T\<^sub>E\<^sub>S\<^sub>L \<union> \<lbrakk>\<lbrakk> \<Gamma> \<rbrakk>\<rbrakk>\<^sub>s\<^sub>y\<^sub>m\<^sub>r\<^sub>u\<^sub>n \<inter> \<lbrakk>\<lbrakk> \<Psi> \<nabla> n \<rbrakk>\<rbrakk>\<^sub>T\<^sub>E\<^sub>S\<^sub>L \<inter> \<lbrakk> K\<^sub>1 sporadic \<tau> on K\<^sub>2 \<nabla> Suc n \<rbrakk>\<^sub>T\<^sub>E\<^sub>S\<^sub>L = \<lbrakk>\<lbrakk> (K\<^sub>1 sporadic \<tau> on K\<^sub>2) # \<Psi> \<nabla> n \<rbrakk>\<rbrakk>\<^sub>T\<^sub>E\<^sub>S\<^sub>L \<inter> \<lbrakk>\<lbrakk> \<Gamma> \<rbrakk>\<rbrakk>\<^sub>s\<^sub>y\<^sub>m\<^sub>r\<^sub>u\<^sub>n"
-        by auto
-      then show ?thesis
-        by auto
-    qed
-  qed
-
-lemma HeronConf_interp_at_index_tagrel_cases:
-  shows "\<lbrakk> \<Gamma>, n \<turnstile> (tag-relation K\<^sub>1 = \<alpha> * K\<^sub>2 + \<beta>) # \<Psi> \<triangleright> \<Phi> \<rbrakk>\<^sub>c\<^sub>o\<^sub>n\<^sub>f
-          = \<lbrakk> (\<tau>\<^sub>v\<^sub>a\<^sub>r(K\<^sub>1, n) \<doteq> \<alpha> * \<tau>\<^sub>v\<^sub>a\<^sub>r(K\<^sub>2, n) + \<beta>) # \<Gamma>, n \<turnstile> \<Psi> \<triangleright> (tag-relation K\<^sub>1 = \<alpha> * K\<^sub>2 + \<beta>) # \<Phi> \<rbrakk>\<^sub>c\<^sub>o\<^sub>n\<^sub>f"
-  proof -
-    have "\<lbrakk> \<Gamma>, n \<turnstile> (tag-relation K\<^sub>1 = \<alpha> * K\<^sub>2 + \<beta>) # \<Psi> \<triangleright> \<Phi> \<rbrakk>\<^sub>c\<^sub>o\<^sub>n\<^sub>f = \<lbrakk>\<lbrakk> \<Gamma> \<rbrakk>\<rbrakk>\<^sub>s\<^sub>y\<^sub>m\<^sub>r\<^sub>u\<^sub>n \<inter> \<lbrakk>\<lbrakk> (tag-relation K\<^sub>1 = \<alpha> * K\<^sub>2 + \<beta>) # \<Psi> \<nabla> n \<rbrakk>\<rbrakk>\<^sub>T\<^sub>E\<^sub>S\<^sub>L \<inter> \<lbrakk>\<lbrakk> \<Phi> \<nabla> Suc n \<rbrakk>\<rbrakk>\<^sub>T\<^sub>E\<^sub>S\<^sub>L"
-      by simp
-    moreover have "\<lbrakk> (\<tau>\<^sub>v\<^sub>a\<^sub>r(K\<^sub>1, n) \<doteq> \<alpha> * \<tau>\<^sub>v\<^sub>a\<^sub>r(K\<^sub>2, n) + \<beta>) # \<Gamma>, n \<turnstile> \<Psi> \<triangleright> (tag-relation K\<^sub>1 = \<alpha> * K\<^sub>2 + \<beta>) # \<Phi> \<rbrakk>\<^sub>c\<^sub>o\<^sub>n\<^sub>f
-                      = \<lbrakk>\<lbrakk> (\<tau>\<^sub>v\<^sub>a\<^sub>r(K\<^sub>1, n) \<doteq> \<alpha> * \<tau>\<^sub>v\<^sub>a\<^sub>r(K\<^sub>2, n) + \<beta>) # \<Gamma> \<rbrakk>\<rbrakk>\<^sub>s\<^sub>y\<^sub>m\<^sub>r\<^sub>u\<^sub>n \<inter> \<lbrakk>\<lbrakk> \<Psi> \<nabla> n \<rbrakk>\<rbrakk>\<^sub>T\<^sub>E\<^sub>S\<^sub>L \<inter> \<lbrakk>\<lbrakk> (tag-relation K\<^sub>1 = \<alpha> * K\<^sub>2 + \<beta>) # \<Phi> \<nabla> Suc n \<rbrakk>\<rbrakk>\<^sub>T\<^sub>E\<^sub>S\<^sub>L"
-      by simp
-    ultimately show ?thesis
-    proof -
-      have "\<lbrakk> \<tau>\<^sub>v\<^sub>a\<^sub>r (K\<^sub>1, n) \<doteq> \<alpha> * \<tau>\<^sub>v\<^sub>a\<^sub>r (K\<^sub>2, n) + \<beta> \<rbrakk>\<^sub>s\<^sub>y\<^sub>m\<^sub>r\<^sub>u\<^sub>n \<inter> \<lbrakk> tag-relation K\<^sub>1 = \<alpha> * K\<^sub>2 + \<beta> \<nabla> Suc n \<rbrakk>\<^sub>T\<^sub>E\<^sub>S\<^sub>L \<inter> \<lbrakk>\<lbrakk> \<Psi> \<nabla> n \<rbrakk>\<rbrakk>\<^sub>T\<^sub>E\<^sub>S\<^sub>L = \<lbrakk>\<lbrakk> (tag-relation K\<^sub>1 = \<alpha> * K\<^sub>2 + \<beta>) # \<Psi> \<nabla> n \<rbrakk>\<rbrakk>\<^sub>T\<^sub>E\<^sub>S\<^sub>L"
-        using TESL_interp_at_index_tagrel_cases TESL_interpretation_at_index_cons_morph by blast
-      then show ?thesis
-        by auto
-    qed
-  qed
-
-lemma HeronConf_interp_at_index_implies_cases:
-  shows "\<lbrakk> \<Gamma>, n \<turnstile> (K\<^sub>1 implies K\<^sub>2) # \<Psi> \<triangleright> \<Phi> \<rbrakk>\<^sub>c\<^sub>o\<^sub>n\<^sub>f
-          = \<lbrakk> K\<^sub>1 \<not>\<Up> n # \<Gamma>, n \<turnstile> \<Psi> \<triangleright> (K\<^sub>1 implies K\<^sub>2) # \<Phi> \<rbrakk>\<^sub>c\<^sub>o\<^sub>n\<^sub>f
-          \<union> \<lbrakk> K\<^sub>1 \<Up> n # K\<^sub>2 \<Up> n # \<Gamma>, n \<turnstile> \<Psi> \<triangleright> (K\<^sub>1 implies K\<^sub>2) # \<Phi> \<rbrakk>\<^sub>c\<^sub>o\<^sub>n\<^sub>f"
-  proof -
-    have "\<lbrakk> \<Gamma>, n \<turnstile> (K\<^sub>1 implies K\<^sub>2) # \<Psi> \<triangleright> \<Phi> \<rbrakk>\<^sub>c\<^sub>o\<^sub>n\<^sub>f = \<lbrakk>\<lbrakk> \<Gamma> \<rbrakk>\<rbrakk>\<^sub>s\<^sub>y\<^sub>m\<^sub>r\<^sub>u\<^sub>n \<inter> \<lbrakk>\<lbrakk> (K\<^sub>1 implies K\<^sub>2) # \<Psi> \<nabla> n \<rbrakk>\<rbrakk>\<^sub>T\<^sub>E\<^sub>S\<^sub>L \<inter> \<lbrakk>\<lbrakk> \<Phi> \<nabla> Suc n \<rbrakk>\<rbrakk>\<^sub>T\<^sub>E\<^sub>S\<^sub>L"
-      by simp
-    moreover have "\<lbrakk> K\<^sub>1 \<not>\<Up> n # \<Gamma>, n \<turnstile> \<Psi> \<triangleright> (K\<^sub>1 implies K\<^sub>2) # \<Phi> \<rbrakk>\<^sub>c\<^sub>o\<^sub>n\<^sub>f = \<lbrakk>\<lbrakk> K\<^sub>1 \<not>\<Up> n # \<Gamma> \<rbrakk>\<rbrakk>\<^sub>s\<^sub>y\<^sub>m\<^sub>r\<^sub>u\<^sub>n \<inter> \<lbrakk>\<lbrakk> \<Psi> \<nabla> n \<rbrakk>\<rbrakk>\<^sub>T\<^sub>E\<^sub>S\<^sub>L \<inter> \<lbrakk>\<lbrakk> (K\<^sub>1 implies K\<^sub>2) # \<Phi> \<nabla> Suc n \<rbrakk>\<rbrakk>\<^sub>T\<^sub>E\<^sub>S\<^sub>L"
-      by simp
-    moreover have "\<lbrakk> K\<^sub>1 \<Up> n # K\<^sub>2 \<Up> n # \<Gamma>, n \<turnstile> \<Psi> \<triangleright> (K\<^sub>1 implies K\<^sub>2) # \<Phi> \<rbrakk>\<^sub>c\<^sub>o\<^sub>n\<^sub>f = \<lbrakk>\<lbrakk> K\<^sub>1 \<Up> n # K\<^sub>2 \<Up> n # \<Gamma> \<rbrakk>\<rbrakk>\<^sub>s\<^sub>y\<^sub>m\<^sub>r\<^sub>u\<^sub>n \<inter> \<lbrakk>\<lbrakk> \<Psi> \<nabla> n \<rbrakk>\<rbrakk>\<^sub>T\<^sub>E\<^sub>S\<^sub>L \<inter> \<lbrakk>\<lbrakk> (K\<^sub>1 implies K\<^sub>2) # \<Phi> \<nabla> Suc n \<rbrakk>\<rbrakk>\<^sub>T\<^sub>E\<^sub>S\<^sub>L"
-      by simp
-    ultimately show ?thesis
-    proof -
-      have f1: "(\<lbrakk> K\<^sub>1 \<not>\<Up> n \<rbrakk>\<^sub>s\<^sub>y\<^sub>m\<^sub>r\<^sub>u\<^sub>n \<union> \<lbrakk> K\<^sub>1 \<Up> n \<rbrakk>\<^sub>s\<^sub>y\<^sub>m\<^sub>r\<^sub>u\<^sub>n \<inter> \<lbrakk> K\<^sub>2 \<Up> n \<rbrakk>\<^sub>s\<^sub>y\<^sub>m\<^sub>r\<^sub>u\<^sub>n) \<inter> \<lbrakk> K\<^sub>1 implies K\<^sub>2 \<nabla> Suc n \<rbrakk>\<^sub>T\<^sub>E\<^sub>S\<^sub>L \<inter> (\<lbrakk>\<lbrakk> \<Psi> \<nabla> n \<rbrakk>\<rbrakk>\<^sub>T\<^sub>E\<^sub>S\<^sub>L \<inter> \<lbrakk>\<lbrakk> \<Phi> \<nabla> Suc n \<rbrakk>\<rbrakk>\<^sub>T\<^sub>E\<^sub>S\<^sub>L) = \<lbrakk>\<lbrakk> (K\<^sub>1 implies K\<^sub>2) # \<Psi> \<nabla> n \<rbrakk>\<rbrakk>\<^sub>T\<^sub>E\<^sub>S\<^sub>L \<inter> \<lbrakk>\<lbrakk> \<Phi> \<nabla> Suc n \<rbrakk>\<rbrakk>\<^sub>T\<^sub>E\<^sub>S\<^sub>L"
-        using TESL_interp_at_index_implies_cases TESL_interpretation_at_index_cons_morph by blast
-      have "\<lbrakk> K\<^sub>1 \<not>\<Up> n \<rbrakk>\<^sub>s\<^sub>y\<^sub>m\<^sub>r\<^sub>u\<^sub>n \<inter> \<lbrakk>\<lbrakk> \<Gamma> \<rbrakk>\<rbrakk>\<^sub>s\<^sub>y\<^sub>m\<^sub>r\<^sub>u\<^sub>n \<union> \<lbrakk> K\<^sub>1 \<Up> n \<rbrakk>\<^sub>s\<^sub>y\<^sub>m\<^sub>r\<^sub>u\<^sub>n \<inter> \<lbrakk>\<lbrakk> K\<^sub>2 \<Up> n # \<Gamma> \<rbrakk>\<rbrakk>\<^sub>s\<^sub>y\<^sub>m\<^sub>r\<^sub>u\<^sub>n = (\<lbrakk> K\<^sub>1 \<not>\<Up> n \<rbrakk>\<^sub>s\<^sub>y\<^sub>m\<^sub>r\<^sub>u\<^sub>n \<union> \<lbrakk> K\<^sub>1 \<Up> n \<rbrakk>\<^sub>s\<^sub>y\<^sub>m\<^sub>r\<^sub>u\<^sub>n \<inter> \<lbrakk> K\<^sub>2 \<Up> n \<rbrakk>\<^sub>s\<^sub>y\<^sub>m\<^sub>r\<^sub>u\<^sub>n) \<inter> \<lbrakk>\<lbrakk> \<Gamma> \<rbrakk>\<rbrakk>\<^sub>s\<^sub>y\<^sub>m\<^sub>r\<^sub>u\<^sub>n"
-        by force
-      then have "\<lbrakk> \<Gamma>, n \<turnstile> (K\<^sub>1 implies K\<^sub>2) # \<Psi> \<triangleright> \<Phi> \<rbrakk>\<^sub>c\<^sub>o\<^sub>n\<^sub>f = (\<lbrakk> K\<^sub>1 \<not>\<Up> n \<rbrakk>\<^sub>s\<^sub>y\<^sub>m\<^sub>r\<^sub>u\<^sub>n \<inter> \<lbrakk>\<lbrakk> \<Gamma> \<rbrakk>\<rbrakk>\<^sub>s\<^sub>y\<^sub>m\<^sub>r\<^sub>u\<^sub>n \<union> \<lbrakk> K\<^sub>1 \<Up> n \<rbrakk>\<^sub>s\<^sub>y\<^sub>m\<^sub>r\<^sub>u\<^sub>n \<inter> \<lbrakk>\<lbrakk> K\<^sub>2 \<Up> n # \<Gamma> \<rbrakk>\<rbrakk>\<^sub>s\<^sub>y\<^sub>m\<^sub>r\<^sub>u\<^sub>n) \<inter> (\<lbrakk>\<lbrakk> \<Psi> \<nabla> n \<rbrakk>\<rbrakk>\<^sub>T\<^sub>E\<^sub>S\<^sub>L \<inter> \<lbrakk>\<lbrakk> (K\<^sub>1 implies K\<^sub>2) # \<Phi> \<nabla> Suc n \<rbrakk>\<rbrakk>\<^sub>T\<^sub>E\<^sub>S\<^sub>L)"
-        using f1 by (simp add: inf_left_commute inf_sup_aci(2))
-      then show ?thesis
-        by (simp add: Int_Un_distrib2 inf_sup_aci(2))
-    qed
-  qed
-
-lemma HeronConf_interp_at_index_timedelayed_cases:
-  shows "\<lbrakk> \<Gamma>, n \<turnstile> (K\<^sub>1 time-delayed by \<delta>\<tau> on K\<^sub>2 implies K\<^sub>3) # \<Psi> \<triangleright> \<Phi> \<rbrakk>\<^sub>c\<^sub>o\<^sub>n\<^sub>f
-          = \<lbrakk> K\<^sub>1 \<not>\<Up> n # \<Gamma>, n \<turnstile> \<Psi> \<triangleright> (K\<^sub>1 time-delayed by \<delta>\<tau> on K\<^sub>2 implies K\<^sub>3) # \<Phi> \<rbrakk>\<^sub>c\<^sub>o\<^sub>n\<^sub>f
-          \<union> \<lbrakk> K\<^sub>1 \<Up> n # \<Gamma>, n \<turnstile> (K\<^sub>3 sporadic \<lfloor>\<tau>\<^sub>v\<^sub>a\<^sub>r(K\<^sub>2, n) \<oplus> \<delta>\<tau>\<rfloor> on K\<^sub>2) # \<Psi> \<triangleright> (K\<^sub>1 time-delayed by \<delta>\<tau> on K\<^sub>2 implies K\<^sub>3) # \<Phi> \<rbrakk>\<^sub>c\<^sub>o\<^sub>n\<^sub>f"
-  proof -
-    have "\<lbrakk> \<Gamma>, n \<turnstile> (K\<^sub>1 time-delayed by \<delta>\<tau> on K\<^sub>2 implies K\<^sub>3) # \<Psi> \<triangleright> \<Phi> \<rbrakk>\<^sub>c\<^sub>o\<^sub>n\<^sub>f
-           = \<lbrakk>\<lbrakk> \<Gamma> \<rbrakk>\<rbrakk>\<^sub>s\<^sub>y\<^sub>m\<^sub>r\<^sub>u\<^sub>n \<inter> \<lbrakk>\<lbrakk> (K\<^sub>1 time-delayed by \<delta>\<tau> on K\<^sub>2 implies K\<^sub>3) # \<Psi> \<nabla> n \<rbrakk>\<rbrakk>\<^sub>T\<^sub>E\<^sub>S\<^sub>L \<inter> \<lbrakk>\<lbrakk> \<Phi> \<nabla> Suc n \<rbrakk>\<rbrakk>\<^sub>T\<^sub>E\<^sub>S\<^sub>L"
-      by simp
-    moreover have "\<lbrakk> K\<^sub>1 \<not>\<Up> n # \<Gamma>, n \<turnstile> \<Psi> \<triangleright> (K\<^sub>1 time-delayed by \<delta>\<tau> on K\<^sub>2 implies K\<^sub>3) # \<Phi> \<rbrakk>\<^sub>c\<^sub>o\<^sub>n\<^sub>f
-                     = \<lbrakk>\<lbrakk> K\<^sub>1 \<not>\<Up> n # \<Gamma> \<rbrakk>\<rbrakk>\<^sub>s\<^sub>y\<^sub>m\<^sub>r\<^sub>u\<^sub>n \<inter> \<lbrakk>\<lbrakk> \<Psi> \<nabla> n \<rbrakk>\<rbrakk>\<^sub>T\<^sub>E\<^sub>S\<^sub>L \<inter> \<lbrakk>\<lbrakk> (K\<^sub>1 time-delayed by \<delta>\<tau> on K\<^sub>2 implies K\<^sub>3) # \<Phi> \<nabla> Suc n \<rbrakk>\<rbrakk>\<^sub>T\<^sub>E\<^sub>S\<^sub>L"
-      by simp
-    moreover have "\<lbrakk> K\<^sub>1 \<Up> n # \<Gamma>, n \<turnstile> (K\<^sub>3 sporadic \<lfloor>\<tau>\<^sub>v\<^sub>a\<^sub>r(K\<^sub>2, n) \<oplus> \<delta>\<tau>\<rfloor> on K\<^sub>2) # \<Psi> \<triangleright> (K\<^sub>1 time-delayed by \<delta>\<tau> on K\<^sub>2 implies K\<^sub>3) # \<Phi> \<rbrakk>\<^sub>c\<^sub>o\<^sub>n\<^sub>f
-                     = \<lbrakk>\<lbrakk> K\<^sub>1 \<Up> n # \<Gamma> \<rbrakk>\<rbrakk>\<^sub>s\<^sub>y\<^sub>m\<^sub>r\<^sub>u\<^sub>n \<inter> \<lbrakk>\<lbrakk> (K\<^sub>3 sporadic \<lfloor>\<tau>\<^sub>v\<^sub>a\<^sub>r(K\<^sub>2, n) \<oplus> \<delta>\<tau>\<rfloor> on K\<^sub>2) # \<Psi> \<nabla> n \<rbrakk>\<rbrakk>\<^sub>T\<^sub>E\<^sub>S\<^sub>L
-                     \<inter> \<lbrakk>\<lbrakk> (K\<^sub>1 time-delayed by \<delta>\<tau> on K\<^sub>2 implies K\<^sub>3) # \<Phi> \<nabla> Suc n \<rbrakk>\<rbrakk>\<^sub>T\<^sub>E\<^sub>S\<^sub>L"
-      by simp
-    ultimately show ?thesis
-    proof -
-      have "\<lbrakk> \<Gamma>, n \<turnstile> (K\<^sub>1 time-delayed by \<delta>\<tau> on K\<^sub>2 implies K\<^sub>3) # \<Psi> \<triangleright> \<Phi> \<rbrakk>\<^sub>c\<^sub>o\<^sub>n\<^sub>f = \<lbrakk>\<lbrakk> \<Gamma> \<rbrakk>\<rbrakk>\<^sub>s\<^sub>y\<^sub>m\<^sub>r\<^sub>u\<^sub>n \<inter> (\<lbrakk>\<lbrakk> (K\<^sub>1 time-delayed by \<delta>\<tau> on K\<^sub>2 implies K\<^sub>3) # \<Psi> \<nabla> n \<rbrakk>\<rbrakk>\<^sub>T\<^sub>E\<^sub>S\<^sub>L \<inter> \<lbrakk>\<lbrakk> \<Phi> \<nabla> Suc n \<rbrakk>\<rbrakk>\<^sub>T\<^sub>E\<^sub>S\<^sub>L)"
-        using \<open>\<lbrakk> \<Gamma>, n \<turnstile> (K\<^sub>1 time-delayed by \<delta>\<tau> on K\<^sub>2 implies K\<^sub>3) # \<Psi> \<triangleright> \<Phi> \<rbrakk>\<^sub>c\<^sub>o\<^sub>n\<^sub>f = \<lbrakk>\<lbrakk> \<Gamma> \<rbrakk>\<rbrakk>\<^sub>s\<^sub>y\<^sub>m\<^sub>r\<^sub>u\<^sub>n \<inter> \<lbrakk>\<lbrakk> (K\<^sub>1 time-delayed by \<delta>\<tau> on K\<^sub>2 implies K\<^sub>3) # \<Psi> \<nabla> n \<rbrakk>\<rbrakk>\<^sub>T\<^sub>E\<^sub>S\<^sub>L \<inter> \<lbrakk>\<lbrakk> \<Phi> \<nabla> Suc n \<rbrakk>\<rbrakk>\<^sub>T\<^sub>E\<^sub>S\<^sub>L\<close> by blast
-      then have "\<lbrakk> \<Gamma>, n \<turnstile> (K\<^sub>1 time-delayed by \<delta>\<tau> on K\<^sub>2 implies K\<^sub>3) # \<Psi> \<triangleright> \<Phi> \<rbrakk>\<^sub>c\<^sub>o\<^sub>n\<^sub>f = (\<lbrakk> K\<^sub>1 \<not>\<Up> n \<rbrakk>\<^sub>s\<^sub>y\<^sub>m\<^sub>r\<^sub>u\<^sub>n \<union> \<lbrakk> K\<^sub>1 \<Up> n \<rbrakk>\<^sub>s\<^sub>y\<^sub>m\<^sub>r\<^sub>u\<^sub>n \<inter> \<lbrakk> K\<^sub>3 sporadic \<lfloor> \<tau>\<^sub>v\<^sub>a\<^sub>r (K\<^sub>2, n) \<oplus> \<delta>\<tau> \<rfloor> on K\<^sub>2 \<nabla> n \<rbrakk>\<^sub>T\<^sub>E\<^sub>S\<^sub>L) \<inter> (\<lbrakk>\<lbrakk> \<Gamma> \<rbrakk>\<rbrakk>\<^sub>s\<^sub>y\<^sub>m\<^sub>r\<^sub>u\<^sub>n \<inter> (\<lbrakk>\<lbrakk> \<Psi> \<nabla> n \<rbrakk>\<rbrakk>\<^sub>T\<^sub>E\<^sub>S\<^sub>L \<inter> \<lbrakk>\<lbrakk> (K\<^sub>1 time-delayed by \<delta>\<tau> on K\<^sub>2 implies K\<^sub>3) # \<Phi> \<nabla> Suc n \<rbrakk>\<rbrakk>\<^sub>T\<^sub>E\<^sub>S\<^sub>L))"
-        using TESL_interp_at_index_timedelayed_cases TESL_interpretation_at_index_cons_morph by blast
-      then show ?thesis
-        by auto
-    qed
-  qed
+  by (simp add: operational_semantics_step.simps operational_semantics_elim.timedelayed_e1 operational_semantics_elim.timedelayed_e2)
 
 inductive finite_SAT :: "config \<Rightarrow> bool" ("\<TTurnstile> _" 50) where
   finite_SAT_ax: "set (NoSporadic \<Phi>) = set \<Phi> \<Longrightarrow>
